@prefix : <http://example.org/virtualhome2kg/ontology/> .
@prefix ho: <http://www.owl-ontologies.com/VirtualHome.owl#> .
@prefix owl: <http://www.w3.org/2002/07/owl#> .
@prefix rdf: <http://www.w3.org/1999/02/22-rdf-syntax-ns#> .
@prefix xml: <http://www.w3.org/XML/1998/namespace> .
@prefix xsd: <http://www.w3.org/2001/XMLSchema#> .
@prefix rdfs: <http://www.w3.org/2000/01/rdf-schema#> .
@prefix x3do: <https://www.web3d.org/specifications/X3dOntology4.0#> .
@base <http://example.org/virtualhome2kg/ontology/> .

<http://example.org/virtualhome2kg/ontology/> rdf:type owl:Ontology ;
                                               rdfs:comment """This ontology offers vocabularies for representing activities of daily living (ADL) that can be run in the VirtualHome (http://virtual-home.org/), run-time home situations, objects, and relationships among them.
This ontology is an extended version of the HomeOntology (https://github.com/valexande/HomeOntology).""" .

#################################################################
#    Annotation properties
#################################################################

###  http://purl.org/dc/terms/description
<http://purl.org/dc/terms/description> rdf:type owl:AnnotationProperty .


#################################################################
#    Datatypes
#################################################################

###  https://www.web3d.org/specifications/X3dOntology4.0#SFDouble
x3do:SFDouble rdf:type rdfs:Datatype .


###  https://www.web3d.org/specifications/X3dOntology4.0#SFVec3f
x3do:SFVec3f rdf:type rdfs:Datatype .


#################################################################
#    Object Properties
#################################################################

###  http://example.org/virtualhome2kg/ontology/action
:action rdf:type owl:ObjectProperty ;
        rdfs:domain ho:Activity ;
        rdfs:range :Action .


###  http://example.org/virtualhome2kg/ontology/activity
:activity rdf:type owl:ObjectProperty ;
          rdfs:domain :Character ;
          rdfs:range ho:Activity .


###  http://example.org/virtualhome2kg/ontology/affordAction
:affordAction rdf:type owl:ObjectProperty ;
              rdfs:range :Action .


###  http://example.org/virtualhome2kg/ontology/affordance
:affordance rdf:type owl:ObjectProperty ;
            rdfs:domain :State ;
            rdfs:range :Affordance .


###  http://example.org/virtualhome2kg/ontology/agent
:agent rdf:type owl:ObjectProperty ;
       rdfs:range :Character .


###  http://example.org/virtualhome2kg/ontology/attribute
:attribute rdf:type owl:ObjectProperty ;
           rdfs:range :Attribute .


###  http://example.org/virtualhome2kg/ontology/bbox
:bbox rdf:type owl:ObjectProperty ;
      rdfs:domain :State ;
      rdfs:range x3do:Shape ;
      rdfs:comment "3D bounding box" .


###  http://example.org/virtualhome2kg/ontology/between
:between rdf:type owl:ObjectProperty ;
         rdfs:subPropertyOf :relatedShape ;
         rdfs:domain x3do:Shape ;
         rdfs:range x3do:Shape ;
         rdfs:comment "used for door object, if door is between kitchen and livingroom, we have edges <door, between, livingroom> and <door, between ,kitchen>" .


###  http://example.org/virtualhome2kg/ontology/close
:close rdf:type owl:ObjectProperty ;
       rdfs:subPropertyOf :relatedShape ;
       rdfs:domain x3do:Shape ;
       rdfs:range x3do:Shape ;
       rdfs:comment "edge <object1, close, object2> denotes that the distance between center of object1 (object2) to the bounding box of object2 (object1) is < 1.5 units (~meters)" .


###  http://example.org/virtualhome2kg/ontology/facing
:facing rdf:type owl:ObjectProperty ;
        rdfs:subPropertyOf :relatedShape ;
        rdfs:domain x3do:Shape ;
        rdfs:range x3do:Shape ;
        rdfs:comment "there is an edge <object1, facing, object2> if object2 is lookable, is visible from object1, and the distance between the centers is < 5 units (~meters). If object1 is a sofa or a chair it should also be turned towards object2" .


###  http://example.org/virtualhome2kg/ontology/holds_lh
:holds_lh rdf:type owl:ObjectProperty ;
          rdfs:subPropertyOf :relatedShape ;
          rdfs:domain x3do:Shape ;
          rdfs:range x3do:Shape ;
          rdfs:comment "analogue of holds_rh for left hand" .


###  http://example.org/virtualhome2kg/ontology/holds_rh
:holds_rh rdf:type owl:ObjectProperty ;
          rdfs:subPropertyOf :relatedShape ;
          rdfs:domain x3do:Shape ;
          rdfs:range x3do:Shape ;
          rdfs:comment "edge <character, holds_rh, object> is used to indicate that character holds an object in its right hand" .


###  http://example.org/virtualhome2kg/ontology/inside
:inside rdf:type owl:ObjectProperty ;
        rdfs:subPropertyOf :relatedShape ;
        rdfs:domain x3do:Shape ;
        rdfs:range x3do:Shape .


###  http://example.org/virtualhome2kg/ontology/isStateOf
:isStateOf rdf:type owl:ObjectProperty ;
           rdfs:domain :State ;
           rdfs:range :Object .


###  http://example.org/virtualhome2kg/ontology/nextAction
:nextAction rdf:type owl:ObjectProperty ;
            rdfs:subPropertyOf :relatedAction ;
            owl:inverseOf :previousAction ;
            rdfs:domain :Action ;
            rdfs:range :Action .


###  http://example.org/virtualhome2kg/ontology/nextActivity
:nextActivity rdf:type owl:ObjectProperty ;
              rdfs:subPropertyOf :relatedActivity ;
              rdfs:domain ho:Activity ;
              rdfs:range ho:Activity .


###  http://example.org/virtualhome2kg/ontology/nextSituation
:nextSituation rdf:type owl:ObjectProperty ;
               rdfs:subPropertyOf :relatedSituation ;
               owl:inverseOf :previousSituation ;
               rdfs:domain :Situation ;
               rdfs:range :Situation .


###  http://example.org/virtualhome2kg/ontology/nextState
:nextState rdf:type owl:ObjectProperty ;
           rdfs:subPropertyOf :relatedState ;
           owl:inverseOf :previousState ;
           rdfs:domain :State ;
           rdfs:range :State .


###  http://example.org/virtualhome2kg/ontology/on
:on rdf:type owl:ObjectProperty ;
    rdfs:subPropertyOf :relatedShape ;
    rdfs:domain x3do:Shape ;
    rdfs:range x3do:Shape .


###  http://example.org/virtualhome2kg/ontology/partOf
:partOf rdf:type owl:ObjectProperty ;
        rdfs:domain :State ;
        rdfs:range :Situation .


###  http://example.org/virtualhome2kg/ontology/previousAction
:previousAction rdf:type owl:ObjectProperty ;
                rdfs:subPropertyOf :relatedAction ;
                rdfs:domain :Action ;
                rdfs:range :Action .


###  http://example.org/virtualhome2kg/ontology/previousActivity
:previousActivity rdf:type owl:ObjectProperty ;
                  rdfs:subPropertyOf :relatedActivity .


###  http://example.org/virtualhome2kg/ontology/previousSituation
:previousSituation rdf:type owl:ObjectProperty ;
                   rdfs:subPropertyOf :relatedSituation ;
                   rdfs:domain :Situation ;
                   rdfs:range :Situation .


###  http://example.org/virtualhome2kg/ontology/previousState
:previousState rdf:type owl:ObjectProperty ;
               rdfs:subPropertyOf :relatedState ;
               rdfs:domain :State ;
               rdfs:range :State .


###  http://example.org/virtualhome2kg/ontology/relatedAction
:relatedAction rdf:type owl:ObjectProperty ;
               rdfs:range :Action .


###  http://example.org/virtualhome2kg/ontology/relatedActivity
:relatedActivity rdf:type owl:ObjectProperty ;
                 rdfs:range ho:Activity .


###  http://example.org/virtualhome2kg/ontology/relatedShape
:relatedShape rdf:type owl:ObjectProperty ;
              rdfs:range x3do:Shape .


###  http://example.org/virtualhome2kg/ontology/relatedSituation
:relatedSituation rdf:type owl:ObjectProperty ;
                  rdfs:range :Situation .


###  http://example.org/virtualhome2kg/ontology/relatedState
:relatedState rdf:type owl:ObjectProperty ;
              rdfs:range :State .


###  http://example.org/virtualhome2kg/ontology/situationAfterAction
:situationAfterAction rdf:type owl:ObjectProperty ;
                      rdfs:subPropertyOf :relatedSituation ;
                      owl:inverseOf :situationBeforeAction ;
                      rdfs:range :Situation .


###  http://example.org/virtualhome2kg/ontology/situationBeforeAction
:situationBeforeAction rdf:type owl:ObjectProperty ;
                       rdfs:subPropertyOf :relatedSituation ;
                       rdfs:range :Situation .


###  http://example.org/virtualhome2kg/ontology/state
:state rdf:type owl:ObjectProperty ;
       rdfs:domain :State ;
       rdfs:range :StateType .


###  http://example.org/virtualhome2kg/ontology/virtualHome
:virtualHome rdf:type owl:ObjectProperty ;
             rdfs:range :VirtualHome .


###  http://www.owl-ontologies.com/VirtualHome.owl#object
ho:object rdf:type owl:ObjectProperty ;
          rdfs:domain :Action ;
          rdfs:range :Object .


###  http://www.w3.org/2006/time#hasDuration
<http://www.w3.org/2006/time#hasDuration> rdf:type owl:ObjectProperty ;
                                          rdfs:range <http://www.w3.org/2006/time#Duration> .


###  http://www.w3.org/2006/time#unitType
<http://www.w3.org/2006/time#unitType> rdf:type owl:ObjectProperty ;
                                       rdfs:range <http://www.w3.org/2006/time#TemporalUnit> .


#################################################################
#    Data properties
#################################################################

###  http://example.org/virtualhome2kg/ontology/actionNumber
:actionNumber rdf:type owl:DatatypeProperty ;
              rdfs:domain :Action ;
              rdfs:range xsd:int .


###  http://example.org/virtualhome2kg/ontology/activityNumber
:activityNumber rdf:type owl:DatatypeProperty ;
                rdfs:domain ho:Activity ;
                rdfs:range xsd:int .


###  http://www.w3.org/2006/time#numericDuration
<http://www.w3.org/2006/time#numericDuration> rdf:type owl:DatatypeProperty ;
                                              rdfs:range xsd:decimal .


###  https://www.web3d.org/specifications/X3dOntology4.0#bboxCenter
x3do:bboxCenter rdf:type owl:DatatypeProperty ;
                rdfs:domain x3do:Shape ;
                rdfs:range x3do:SFVec3f .


###  https://www.web3d.org/specifications/X3dOntology4.0#bboxSize
x3do:bboxSize rdf:type owl:DatatypeProperty ;
              rdfs:domain x3do:Shape ;
              rdfs:range x3do:SFVec3f .


#################################################################
#    Classes
#################################################################

###  http://example.org/virtualhome2kg/ontology/Action
:Action rdf:type owl:Class .


###  http://example.org/virtualhome2kg/ontology/Affordance
:Affordance rdf:type owl:Class .


###  http://example.org/virtualhome2kg/ontology/Attribute
:Attribute rdf:type owl:Class ;
           rdfs:comment "This class means properties of objects. We do not use 'property' as a class name because 'property' means edges of RDF graphs." .


###  http://example.org/virtualhome2kg/ontology/Break
:Break rdf:type owl:Class ;
       rdfs:subClassOf :Action .


###  http://example.org/virtualhome2kg/ontology/Brush
:Brush rdf:type owl:Class ;
       rdfs:subClassOf :Action .


###  http://example.org/virtualhome2kg/ontology/Call
:Call rdf:type owl:Class ;
      rdfs:subClassOf :Action .


###  http://example.org/virtualhome2kg/ontology/Character
:Character rdf:type owl:Class ;
           rdfs:subClassOf :Object .


###  http://example.org/virtualhome2kg/ontology/Climb
:Climb rdf:type owl:Class ;
       rdfs:subClassOf :Action .


###  http://example.org/virtualhome2kg/ontology/Close
:Close rdf:type owl:Class ;
       rdfs:subClassOf :Action .


###  http://example.org/virtualhome2kg/ontology/Cover
:Cover rdf:type owl:Class ;
       rdfs:subClassOf :Action .


###  http://example.org/virtualhome2kg/ontology/Crawl
:Crawl rdf:type owl:Class ;
       rdfs:subClassOf :Action .


###  http://example.org/virtualhome2kg/ontology/Cut
:Cut rdf:type owl:Class ;
     rdfs:subClassOf :Action .


###  http://example.org/virtualhome2kg/ontology/Dance
:Dance rdf:type owl:Class ;
       rdfs:subClassOf :Action .


###  http://example.org/virtualhome2kg/ontology/Dial
:Dial rdf:type owl:Class ;
      rdfs:subClassOf :Action .


###  http://example.org/virtualhome2kg/ontology/Drink
:Drink rdf:type owl:Class ;
       rdfs:subClassOf :Action .


###  http://example.org/virtualhome2kg/ontology/Drop
:Drop rdf:type owl:Class ;
      rdfs:subClassOf :Action .


###  http://example.org/virtualhome2kg/ontology/Eat
:Eat rdf:type owl:Class ;
     rdfs:subClassOf :Action .


###  http://example.org/virtualhome2kg/ontology/Enter
:Enter rdf:type owl:Class ;
       rdfs:subClassOf :Action .


###  http://example.org/virtualhome2kg/ontology/Find
:Find rdf:type owl:Class ;
      rdfs:subClassOf :Action .


###  http://example.org/virtualhome2kg/ontology/Flush
:Flush rdf:type owl:Class ;
       rdfs:subClassOf :Action .


###  http://example.org/virtualhome2kg/ontology/Fold
:Fold rdf:type owl:Class ;
      rdfs:subClassOf :Action .


###  http://example.org/virtualhome2kg/ontology/Grab
:Grab rdf:type owl:Class ;
      rdfs:subClassOf :Action .


###  http://example.org/virtualhome2kg/ontology/Greet
:Greet rdf:type owl:Class ;
       rdfs:subClassOf :Action .


###  http://example.org/virtualhome2kg/ontology/Jump
:Jump rdf:type owl:Class ;
      rdfs:subClassOf :Action .


###  http://example.org/virtualhome2kg/ontology/Laugh
:Laugh rdf:type owl:Class ;
       rdfs:subClassOf :Action .


###  http://example.org/virtualhome2kg/ontology/Leave
:Leave rdf:type owl:Class ;
       rdfs:subClassOf :Action .


###  http://example.org/virtualhome2kg/ontology/Lie
:Lie rdf:type owl:Class ;
     rdfs:subClassOf :Action .


###  http://example.org/virtualhome2kg/ontology/LookAt
:LookAt rdf:type owl:Class ;
        rdfs:subClassOf :Action .


###  http://example.org/virtualhome2kg/ontology/Move
:Move rdf:type owl:Class ;
      rdfs:subClassOf :Action .


###  http://example.org/virtualhome2kg/ontology/Object
:Object rdf:type owl:Class ;
        rdfs:comment "The class with the object instances from the household environment." .


###  http://example.org/virtualhome2kg/ontology/Open
:Open rdf:type owl:Class ;
      rdfs:subClassOf :Action .


###  http://example.org/virtualhome2kg/ontology/Play
:Play rdf:type owl:Class ;
      rdfs:subClassOf :Action .


###  http://example.org/virtualhome2kg/ontology/PlugIn
:PlugIn rdf:type owl:Class ;
        rdfs:subClassOf :Action .


###  http://example.org/virtualhome2kg/ontology/PlugOut
:PlugOut rdf:type owl:Class ;
         rdfs:subClassOf :Action .


###  http://example.org/virtualhome2kg/ontology/PointAt
:PointAt rdf:type owl:Class ;
         rdfs:subClassOf :Action .


###  http://example.org/virtualhome2kg/ontology/Pour
:Pour rdf:type owl:Class ;
      rdfs:subClassOf :Action .


###  http://example.org/virtualhome2kg/ontology/Pull
:Pull rdf:type owl:Class ;
      rdfs:subClassOf :Action .


###  http://example.org/virtualhome2kg/ontology/Push
:Push rdf:type owl:Class ;
      rdfs:subClassOf :Action .


###  http://example.org/virtualhome2kg/ontology/Put
:Put rdf:type owl:Class ;
     rdfs:subClassOf :Action .


###  http://example.org/virtualhome2kg/ontology/PutBack
:PutBack rdf:type owl:Class ;
         rdfs:subClassOf :Action .


###  http://example.org/virtualhome2kg/ontology/PutIn
:PutIn rdf:type owl:Class ;
       rdfs:subClassOf :Action .


###  http://example.org/virtualhome2kg/ontology/PutObjBack
:PutObjBack rdf:type owl:Class ;
            rdfs:subClassOf :Action .


###  http://example.org/virtualhome2kg/ontology/PutOff
:PutOff rdf:type owl:Class ;
        rdfs:subClassOf :Action .


###  http://example.org/virtualhome2kg/ontology/PutOn
:PutOn rdf:type owl:Class ;
       rdfs:subClassOf :Action .


###  http://example.org/virtualhome2kg/ontology/Read
:Read rdf:type owl:Class ;
      rdfs:subClassOf :Action .


###  http://example.org/virtualhome2kg/ontology/Rinse
:Rinse rdf:type owl:Class ;
       rdfs:subClassOf :Action .


###  http://example.org/virtualhome2kg/ontology/Run
:Run rdf:type owl:Class ;
     rdfs:subClassOf :Action .


###  http://example.org/virtualhome2kg/ontology/Scrub
:Scrub rdf:type owl:Class ;
       rdfs:subClassOf :Action .


###  http://example.org/virtualhome2kg/ontology/Sew
:Sew rdf:type owl:Class ;
     rdfs:subClassOf :Action .


###  http://example.org/virtualhome2kg/ontology/Shake
:Shake rdf:type owl:Class ;
       rdfs:subClassOf :Action .


###  http://example.org/virtualhome2kg/ontology/Sing
:Sing rdf:type owl:Class ;
      rdfs:subClassOf :Action .


###  http://example.org/virtualhome2kg/ontology/Sit
:Sit rdf:type owl:Class ;
     rdfs:subClassOf :Action .


###  http://example.org/virtualhome2kg/ontology/Situation
:Situation rdf:type owl:Class ;
           rdfs:comment "The class which describes the situation of the entire home at a certain moment." .


###  http://example.org/virtualhome2kg/ontology/Sleep
:Sleep rdf:type owl:Class ;
       rdfs:subClassOf :Action .


###  http://example.org/virtualhome2kg/ontology/Soak
:Soak rdf:type owl:Class ;
      rdfs:subClassOf :Action .


###  http://example.org/virtualhome2kg/ontology/Speak
:Speak rdf:type owl:Class ;
       rdfs:subClassOf :Action .


###  http://example.org/virtualhome2kg/ontology/Spit
:Spit rdf:type owl:Class ;
      rdfs:subClassOf :Action .


###  http://example.org/virtualhome2kg/ontology/Spread
:Spread rdf:type owl:Class ;
        rdfs:subClassOf :Action .


###  http://example.org/virtualhome2kg/ontology/Squeeze
:Squeeze rdf:type owl:Class ;
         rdfs:subClassOf :Action .


###  http://example.org/virtualhome2kg/ontology/StandUp
:StandUp rdf:type owl:Class ;
         rdfs:subClassOf :Action .


###  http://example.org/virtualhome2kg/ontology/State
:State rdf:type owl:Class ;
       rdfs:comment "The class which describes the state of the object in the household at a certain moment." .


###  http://example.org/virtualhome2kg/ontology/StateType
:StateType rdf:type owl:Class .


###  http://example.org/virtualhome2kg/ontology/Stir
:Stir rdf:type owl:Class ;
      rdfs:subClassOf :Action .


###  http://example.org/virtualhome2kg/ontology/Stretch
:Stretch rdf:type owl:Class ;
         rdfs:subClassOf :Action .


###  http://example.org/virtualhome2kg/ontology/Sweep
:Sweep rdf:type owl:Class ;
       rdfs:subClassOf :Action .


###  http://example.org/virtualhome2kg/ontology/SwitchOff
:SwitchOff rdf:type owl:Class ;
           rdfs:subClassOf :Action .


###  http://example.org/virtualhome2kg/ontology/SwitchOn
:SwitchOn rdf:type owl:Class ;
          rdfs:subClassOf :Action .


###  http://example.org/virtualhome2kg/ontology/Talk
:Talk rdf:type owl:Class ;
      rdfs:subClassOf :Action .


###  http://example.org/virtualhome2kg/ontology/Text
:Text rdf:type owl:Class ;
      rdfs:subClassOf :Action .


###  http://example.org/virtualhome2kg/ontology/Throw
:Throw rdf:type owl:Class ;
       rdfs:subClassOf :Action .


###  http://example.org/virtualhome2kg/ontology/Touch
:Touch rdf:type owl:Class ;
       rdfs:subClassOf :Action .


###  http://example.org/virtualhome2kg/ontology/TurnTo
:TurnTo rdf:type owl:Class ;
        rdfs:subClassOf :Action .


###  http://example.org/virtualhome2kg/ontology/Type
:Type rdf:type owl:Class ;
      rdfs:subClassOf :Action .


###  http://example.org/virtualhome2kg/ontology/Uncover
:Uncover rdf:type owl:Class ;
         rdfs:subClassOf :Action .


###  http://example.org/virtualhome2kg/ontology/Unfold
:Unfold rdf:type owl:Class ;
        rdfs:subClassOf :Action .


###  http://example.org/virtualhome2kg/ontology/Unwrap
:Unwrap rdf:type owl:Class ;
        rdfs:subClassOf :Action .


###  http://example.org/virtualhome2kg/ontology/Vacuum
:Vacuum rdf:type owl:Class ;
        rdfs:subClassOf :Action .


###  http://example.org/virtualhome2kg/ontology/VirtualHome
:VirtualHome rdf:type owl:Class .


###  http://example.org/virtualhome2kg/ontology/Wait
:Wait rdf:type owl:Class ;
      rdfs:subClassOf :Action .


###  http://example.org/virtualhome2kg/ontology/WakeUp
:WakeUp rdf:type owl:Class ;
        rdfs:subClassOf :Action .


###  http://example.org/virtualhome2kg/ontology/Walk
:Walk rdf:type owl:Class ;
      rdfs:subClassOf :Action .


###  http://example.org/virtualhome2kg/ontology/Watch
:Watch rdf:type owl:Class ;
       rdfs:subClassOf :Action .


###  http://example.org/virtualhome2kg/ontology/Wipe
:Wipe rdf:type owl:Class ;
      rdfs:subClassOf :Action .


###  http://example.org/virtualhome2kg/ontology/Wrap
:Wrap rdf:type owl:Class ;
      rdfs:subClassOf :Action .


###  http://example.org/virtualhome2kg/ontology/Write
:Write rdf:type owl:Class ;
       rdfs:subClassOf :Action .


###  http://www.owl-ontologies.com/VirtualHome.owl#Activity
ho:Activity rdf:type owl:Class ;
            rdfs:subClassOf [ rdf:type owl:Restriction ;
                              owl:onProperty :action ;
                              owl:minQualifiedCardinality "1"^^xsd:nonNegativeInteger ;
                              owl:onClass :Action
                            ] .


###  http://www.owl-ontologies.com/VirtualHome.owl#BedTimeSleep
ho:BedTimeSleep rdf:type owl:Class ;
                rdfs:subClassOf ho:Activity ;
                rdfs:comment """Class with sequences for getting ready for the bed, or get ready for 
sleep, or even put the kids to sleep
.""" .


###  http://www.owl-ontologies.com/VirtualHome.owl#Dance
ho:Dance rdf:type owl:Class ;
         rdfs:subClassOf ho:Leisure ;
         rdfs:comment "The class with sequence of actions for dancing." .


###  http://www.owl-ontologies.com/VirtualHome.owl#Drink
ho:Drink rdf:type owl:Class ;
         rdfs:subClassOf ho:EatingDrinking ;
         rdfs:comment """Class that contains sequences where the goal is for the user to drink 
under different circumstances.""" .


###  http://www.owl-ontologies.com/VirtualHome.owl#Eat
ho:Eat rdf:type owl:Class ;
       rdfs:subClassOf ho:EatingDrinking ;
       rdfs:comment """Class with subclasses, for eating seqeunces under different 
circumstances.""" .


###  http://www.owl-ontologies.com/VirtualHome.owl#EatingDrinking
ho:EatingDrinking rdf:type owl:Class ;
                  rdfs:subClassOf ho:Activity ;
                  rdfs:comment "Class that contains sequences for eating and drinking." .


###  http://www.owl-ontologies.com/VirtualHome.owl#FoodPreparation
ho:FoodPreparation rdf:type owl:Class ;
                   rdfs:subClassOf ho:Activity ;
                   rdfs:comment """Class for preparing food, or other kitchen based acitivities for eating 
or drinking (prepeare coffee).""" .


###  http://www.owl-ontologies.com/VirtualHome.owl#GettingReady
ho:GettingReady rdf:type owl:Class ;
                rdfs:subClassOf ho:Activity ;
                rdfs:comment """Class with sequences for getting ready to go to work, or getting ready 
o perform a task outside the home, or even a procedure that needs prior 
preparation.""" .


###  http://www.owl-ontologies.com/VirtualHome.owl#HouseArrangement
ho:HouseArrangement rdf:type owl:Class ;
                    rdfs:subClassOf ho:Activity ;
                    rdfs:comment "Superclass that contains sequence for arrangement tasks inside the house. Some of these classes could have been classified as a House Cleaning subclass. We prefer this hierarchy, because the task are more to the category of organizing object inside a domestic environment, rather than cleaning." .


###  http://www.owl-ontologies.com/VirtualHome.owl#HouseCleaning
ho:HouseCleaning rdf:type owl:Class ;
                 rdfs:subClassOf ho:Activity ;
                 rdfs:comment "The class that contains sequence of actions, with Cleaning tasks." .


###  http://www.owl-ontologies.com/VirtualHome.owl#HygieneStyling
ho:HygieneStyling rdf:type owl:Class ;
                  rdfs:subClassOf ho:Activity ;
                  rdfs:comment """Class for sequence that are related to Hygiene otr Styling (NOTICE: some 
of this sequences could be conisdered also as cleaning).""" .


###  http://www.owl-ontologies.com/VirtualHome.owl#Laugh
ho:Laugh rdf:type owl:Class ;
         rdfs:subClassOf ho:Other ;
         rdfs:comment "The class with sequence of actions for laughing." .


###  http://www.owl-ontologies.com/VirtualHome.owl#Leisure
ho:Leisure rdf:type owl:Class ;
           rdfs:subClassOf ho:Activity ;
           rdfs:comment "Class that contains procedures about leisure" .


###  http://www.owl-ontologies.com/VirtualHome.owl#Other
ho:Other rdf:type owl:Class ;
         rdfs:subClassOf ho:Activity ;
         rdfs:comment """This class contains instances that are tasks performed inside a domestic 
envronmnet but could not be classified in a specific class.""" .


###  http://www.owl-ontologies.com/VirtualHome.owl#PhysicalActivity
ho:PhysicalActivity rdf:type owl:Class ;
                    rdfs:subClassOf ho:Activity ;
                    rdfs:comment "Class with sequences for exercise and different physical activities." .


###  http://www.owl-ontologies.com/VirtualHome.owl#Play
ho:Play rdf:type owl:Class ;
        rdfs:subClassOf ho:Leisure ;
        rdfs:comment "The class with sequence of actions on how to play (physical games)." .


###  http://www.owl-ontologies.com/VirtualHome.owl#Read
ho:Read rdf:type owl:Class ;
        rdfs:subClassOf ho:Other ;
        rdfs:comment "The class with sequence of actions for  reading." .


###  http://www.owl-ontologies.com/VirtualHome.owl#Sew
ho:Sew rdf:type owl:Class ;
       rdfs:subClassOf ho:Other ;
       rdfs:comment "The class with sequence of actions for sewing, from inside the house." .


###  http://www.owl-ontologies.com/VirtualHome.owl#Shave
ho:Shave rdf:type owl:Class ;
         rdfs:subClassOf ho:HygieneStyling ;
         rdfs:comment "The class with sequence of actions for shaving your own face." .


###  http://www.owl-ontologies.com/VirtualHome.owl#Sit
ho:Sit rdf:type owl:Class ;
       rdfs:subClassOf ho:Other ;
       rdfs:comment "The class with sequence of actions for sitting." .


###  http://www.owl-ontologies.com/VirtualHome.owl#SocialInteraction
ho:SocialInteraction rdf:type owl:Class ;
                     rdfs:subClassOf ho:Activity ;
                     rdfs:comment """Class that contains sequences that are related between , human-robot or 
human-human interaction.""" .


###  http://www.owl-ontologies.com/VirtualHome.owl#Stretch
ho:Stretch rdf:type owl:Class ;
           rdfs:subClassOf ho:PhysicalActivity ;
           rdfs:comment "A class with soft physical activity, or exercise, such as stretch." .


###  http://www.owl-ontologies.com/VirtualHome.owl#Vacuum
ho:Vacuum rdf:type owl:Class ;
          rdfs:subClassOf ho:HouseCleaning ;
          rdfs:comment "Class with sequences on how to vaccum the floor." .


###  http://www.owl-ontologies.com/VirtualHome.owl#Wait
ho:Wait rdf:type owl:Class ;
        rdfs:subClassOf ho:Other ;
        rdfs:comment "The class with sequence of actions for waiting." .


###  http://www.owl-ontologies.com/VirtualHome.owl#Work
ho:Work rdf:type owl:Class ;
        rdfs:subClassOf ho:Activity ;
        rdfs:comment "Class with related activites such as send an email, getting ready for work." .


###  http://www.owl-ontologies.com/VirtualHome.owl#Write
ho:Write rdf:type owl:Class ;
         rdfs:subClassOf ho:Other ;
         rdfs:comment "The class with sequence of actions for writing on a papers or on the computer." .


###  http://www.owl-ontologies.com/VirtualHome.owl#add_paper_to_printer
ho:add_paper_to_printer rdf:type owl:Class ;
                        rdfs:subClassOf ho:Other ;
                        rdfs:comment "The class with sequence of actions for adding paper to the printer." .


###  http://www.owl-ontologies.com/VirtualHome.owl#added_meat_to_freezer
ho:added_meat_to_freezer rdf:type owl:Class ;
                         rdfs:subClassOf ho:HouseArrangement ;
                         rdfs:comment "The class with sequence of actions for adding meat into the freezer." .


###  http://www.owl-ontologies.com/VirtualHome.owl#admire_art
ho:admire_art rdf:type owl:Class ;
              rdfs:subClassOf ho:Other ;
              rdfs:comment """The class with sequence of actions for admiring art that exist inside 
your home.""" .


###  http://www.owl-ontologies.com/VirtualHome.owl#annoy_your_dog
ho:annoy_your_dog rdf:type owl:Class ;
                  rdfs:subClassOf ho:Other ;
                  rdfs:comment "The class with sequence of actions for annoying your dog, in any room (play with dog)." .


###  http://www.owl-ontologies.com/VirtualHome.owl#answer_door
ho:answer_door rdf:type owl:Class ;
               rdfs:subClassOf ho:SocialInteraction ;
               rdfs:comment """The class with sequence of actions for answering the door (main entrance 
of the house).""" .


###  http://www.owl-ontologies.com/VirtualHome.owl#answer_emails
ho:answer_emails rdf:type owl:Class ;
                 rdfs:subClassOf ho:Work ;
                 rdfs:comment """The class with sequence of actions for answering your mails (writing the 
text, not sending the mail).""" .


###  http://www.owl-ontologies.com/VirtualHome.owl#answer_phone
ho:answer_phone rdf:type owl:Class ;
                rdfs:subClassOf ho:Other ;
                rdfs:comment "The class with sequence of actions for answering the phone, cell phone or phone home." .


###  http://www.owl-ontologies.com/VirtualHome.owl#apply_lotion
ho:apply_lotion rdf:type owl:Class ;
                rdfs:subClassOf ho:HygieneStyling ;
                rdfs:comment """The class with sequence of actions for applying lotion in any part of 
the body.""" .


###  http://www.owl-ontologies.com/VirtualHome.owl#arrange_bookshelf
ho:arrange_bookshelf rdf:type owl:Class ;
                     rdfs:subClassOf ho:HouseArrangement ;
                     rdfs:comment "The class with sequence of actions for arranging the bookself." .


###  http://www.owl-ontologies.com/VirtualHome.owl#arrange_folders
ho:arrange_folders rdf:type owl:Class ;
                   rdfs:subClassOf ho:HouseArrangement ;
                   rdfs:comment """The class with sequence of actions for arranging folders, in any place 
or room.""" .


###  http://www.owl-ontologies.com/VirtualHome.owl#arrange_furniture
ho:arrange_furniture rdf:type owl:Class ;
                     rdfs:subClassOf ho:HouseArrangement ;
                     rdfs:comment "The class with sequence of actions for arranging furniture in any room." .


###  http://www.owl-ontologies.com/VirtualHome.owl#arrange_shoes
ho:arrange_shoes rdf:type owl:Class ;
                 rdfs:subClassOf ho:HouseArrangement ;
                 rdfs:comment "The class with sequence of actions for arranging shoes in any room." .


###  http://www.owl-ontologies.com/VirtualHome.owl#arrange_sofa
ho:arrange_sofa rdf:type owl:Class ;
                rdfs:subClassOf ho:HouseArrangement ;
                rdfs:comment "The class with sequence of actions for arranging sofa, in any room." .


###  http://www.owl-ontologies.com/VirtualHome.owl#bake
ho:bake rdf:type owl:Class ;
        rdfs:subClassOf ho:FoodPreparation ;
        rdfs:comment "The class with sequence of actions for baking something." .


###  http://www.owl-ontologies.com/VirtualHome.owl#bathe
ho:bathe rdf:type owl:Class ;
         rdfs:subClassOf ho:HygieneStyling ;
         rdfs:comment "The class with sequence of actions for taking a bathe." .


###  http://www.owl-ontologies.com/VirtualHome.owl#be_able_to_talk_to_me_about_tv_show_im_watching
ho:be_able_to_talk_to_me_about_tv_show_im_watching rdf:type owl:Class ;
                                                   rdfs:subClassOf ho:SocialInteraction ;
                                                   rdfs:comment """The class with sequence of actions for beeing able to talk to the user 
about TV show I'm watching.""" .


###  http://www.owl-ontologies.com/VirtualHome.owl#bed_time
ho:bed_time rdf:type owl:Class ;
            rdfs:subClassOf ho:BedTimeSleep ;
            rdfs:comment "The class with sequence of actions for going to bed." .


###  http://www.owl-ontologies.com/VirtualHome.owl#blow_dry_hair
ho:blow_dry_hair rdf:type owl:Class ;
                 rdfs:subClassOf ho:HygieneStyling ;
                 rdfs:comment "The class with sequence of actions for blowing and drying your hair." .


###  http://www.owl-ontologies.com/VirtualHome.owl#break_table
ho:break_table rdf:type owl:Class ;
               rdfs:subClassOf ho:Other ;
               rdfs:comment "The class with sequence of actions for breaking a table, in any room." .


###  http://www.owl-ontologies.com/VirtualHome.owl#breakfast
ho:breakfast rdf:type owl:Class ;
             rdfs:subClassOf ho:FoodPreparation ;
             rdfs:comment "The class with sequence of actions for breakfast." .


###  http://www.owl-ontologies.com/VirtualHome.owl#brew_coffee
ho:brew_coffee rdf:type owl:Class ;
               rdfs:subClassOf ho:FoodPreparation ;
               rdfs:comment "The class with sequence of actions for brewing coffee in any room." .


###  http://www.owl-ontologies.com/VirtualHome.owl#bring_dirty_plate_to_sink
ho:bring_dirty_plate_to_sink rdf:type owl:Class ;
                             rdfs:subClassOf ho:HouseArrangement ;
                             rdfs:comment """The class with sequence of actions for bringing your dirty plate in the 
sink.""" .


###  http://www.owl-ontologies.com/VirtualHome.owl#bring_food
ho:bring_food rdf:type owl:Class ;
              rdfs:subClassOf ho:Other ;
              rdfs:comment "The class with sequence of actions for bringing food, to home from any place." .


###  http://www.owl-ontologies.com/VirtualHome.owl#bring_leftovers_in_kitchen
ho:bring_leftovers_in_kitchen rdf:type owl:Class ;
                              rdfs:subClassOf ho:HouseArrangement ;
                              rdfs:comment """The class with sequence of actions for bringing leftovers in kitchen, 
from any room.""" .


###  http://www.owl-ontologies.com/VirtualHome.owl#bring_me_red_cookbook
ho:bring_me_red_cookbook rdf:type owl:Class ;
                         rdfs:subClassOf ho:Other ;
                         rdfs:comment """The class with sequence of actions for bringing the user the red 
cookbook.""" .


###  http://www.owl-ontologies.com/VirtualHome.owl#broom
ho:broom rdf:type owl:Class ;
         rdfs:subClassOf ho:HygieneStyling ;
         rdfs:comment "The class with sequence of actions for broomin, every room in the house." .


###  http://www.owl-ontologies.com/VirtualHome.owl#browse_computer
ho:browse_computer rdf:type owl:Class ;
                   rdfs:subClassOf ho:Leisure ;
                   rdfs:comment "The class with sequence of actions for browsing the computer." .


###  http://www.owl-ontologies.com/VirtualHome.owl#browse_internet
ho:browse_internet rdf:type owl:Class ;
                   rdfs:subClassOf ho:Leisure ,
                                   ho:Work ;
                   rdfs:comment "The class which contains sequences for browsing the internet." .


###  http://www.owl-ontologies.com/VirtualHome.owl#brush_hair
ho:brush_hair rdf:type owl:Class ;
              rdfs:subClassOf ho:HygieneStyling ;
              rdfs:comment "The class with sequence of actions for brushing your hair." .


###  http://www.owl-ontologies.com/VirtualHome.owl#brush_teeth
ho:brush_teeth rdf:type owl:Class ;
               rdfs:subClassOf ho:HygieneStyling ;
               rdfs:comment "The class with sequence of actions for brushing your teeth." .


###  http://www.owl-ontologies.com/VirtualHome.owl#build_lego_house
ho:build_lego_house rdf:type owl:Class ;
                    rdfs:subClassOf ho:Other ;
                    rdfs:comment """The class with sequence of actions for building a lego house, in any 
room.""" .


###  http://www.owl-ontologies.com/VirtualHome.owl#call_client
ho:call_client rdf:type owl:Class ;
               rdfs:subClassOf ho:SocialInteraction ;
               rdfs:comment """The class with sequence of actions for calling client, either form cell 
phone or home phone.""" .


###  http://www.owl-ontologies.com/VirtualHome.owl#call_family_member_with_skype_application
ho:call_family_member_with_skype_application rdf:type owl:Class ;
                                             rdfs:subClassOf ho:SocialInteraction ;
                                             rdfs:comment """The class with sequence of actions for calling family member with skype 
application.""" .


###  http://www.owl-ontologies.com/VirtualHome.owl#call_mother
ho:call_mother rdf:type owl:Class ;
               rdfs:subClassOf ho:SocialInteraction ;
               rdfs:comment "The class with sequence of actions for calling your mother." .


###  http://www.owl-ontologies.com/VirtualHome.owl#card
ho:card rdf:type owl:Class ;
        rdfs:subClassOf ho:Other ;
        rdfs:comment "The class with sequence of actions for carding." .


###  http://www.owl-ontologies.com/VirtualHome.owl#care_for_houseplants
ho:care_for_houseplants rdf:type owl:Class ;
                        rdfs:subClassOf ho:HouseArrangement ;
                        rdfs:comment "The class with sequence of actions for for carring for house plants." .


###  http://www.owl-ontologies.com/VirtualHome.owl#carry_groceries_to_kitchen
ho:carry_groceries_to_kitchen rdf:type owl:Class ;
                              rdfs:subClassOf ho:Other ;
                              rdfs:comment "The class with sequence of actions for carrying groceries to kitchen." .


###  http://www.owl-ontologies.com/VirtualHome.owl#celebrate
ho:celebrate rdf:type owl:Class ;
             rdfs:subClassOf ho:Other ;
             rdfs:comment "The class with sequence of actions for celebrating, in any occasion." .


###  http://www.owl-ontologies.com/VirtualHome.owl#celebrate_birthday_with_nice_meal
ho:celebrate_birthday_with_nice_meal rdf:type owl:Class ;
                                     rdfs:subClassOf ho:Other ;
                                     rdfs:comment """The class with sequence of actions for celebrating birthday with a nice 
meal, in any room.""" .


###  http://www.owl-ontologies.com/VirtualHome.owl#change_bedding
ho:change_bedding rdf:type owl:Class ;
                  rdfs:subClassOf ho:HouseArrangement ;
                  rdfs:comment """The class with sequence of actions for changing the bedding, in any bed 
in the house.""" .


###  http://www.owl-ontologies.com/VirtualHome.owl#change_clothes
ho:change_clothes rdf:type owl:Class ;
                  rdfs:subClassOf ho:HygieneStyling ;
                  rdfs:comment "The class with sequence of actions for changing your own clothes." .


###  http://www.owl-ontologies.com/VirtualHome.owl#change_curtains
ho:change_curtains rdf:type owl:Class ;
                   rdfs:subClassOf ho:HouseArrangement ;
                   rdfs:comment "The class with sequence of actions for changing curtains, in any room." .


###  http://www.owl-ontologies.com/VirtualHome.owl#change_light
ho:change_light rdf:type owl:Class ;
                rdfs:subClassOf ho:HouseArrangement ;
                rdfs:comment "The class with sequence of actions for changing lights in any room." .


###  http://www.owl-ontologies.com/VirtualHome.owl#change_lightbulb
ho:change_lightbulb rdf:type owl:Class ;
                    rdfs:subClassOf ho:HouseArrangement ;
                    rdfs:comment "The class with sequence of actions for changing any lightbulb, inside the house." .


###  http://www.owl-ontologies.com/VirtualHome.owl#change_sheets_and_pillow_cases
ho:change_sheets_and_pillow_cases rdf:type owl:Class ;
                                  rdfs:subClassOf ho:HouseArrangement ;
                                  rdfs:comment "The class with sequence of actions for changing sheets and pillow cases, for any bed in the house." .


###  http://www.owl-ontologies.com/VirtualHome.owl#change_sheets_on_bed
ho:change_sheets_on_bed rdf:type owl:Class ;
                        rdfs:subClassOf ho:HouseArrangement ;
                        rdfs:comment "The class with sequence of actions for changing sheets on bed." .


###  http://www.owl-ontologies.com/VirtualHome.owl#change_shower_curtain
ho:change_shower_curtain rdf:type owl:Class ;
                         rdfs:subClassOf ho:HouseArrangement ;
                         rdfs:comment "The class with sequence of actions for changing the curtain from a shower." .


###  http://www.owl-ontologies.com/VirtualHome.owl#change_toilet_paper_roll
ho:change_toilet_paper_roll rdf:type owl:Class ;
                            rdfs:subClassOf ho:HouseArrangement ;
                            rdfs:comment "The class with sequence of actions for changing toilet paper roll." .


###  http://www.owl-ontologies.com/VirtualHome.owl#change_toothbrush
ho:change_toothbrush rdf:type owl:Class ;
                     rdfs:subClassOf ho:HouseArrangement ;
                     rdfs:comment """The class with sequence of actions for changing the toothbrush, in any 
room.""" .


###  http://www.owl-ontologies.com/VirtualHome.owl#change_tv_channel
ho:change_tv_channel rdf:type owl:Class ;
                     rdfs:subClassOf ho:Other ;
                     rdfs:comment "The class with sequence of actions for changing the tv channel." .


###  http://www.owl-ontologies.com/VirtualHome.owl#change_tv_channels
ho:change_tv_channels rdf:type owl:Class ;
                      rdfs:subClassOf ho:Leisure ;
                      rdfs:comment "The class with sequence of actions for changing TV channels." .


###  http://www.owl-ontologies.com/VirtualHome.owl#check_appearance_in_mirror
ho:check_appearance_in_mirror rdf:type owl:Class ;
                              rdfs:subClassOf ho:HygieneStyling ;
                              rdfs:comment "The class with sequence of actions for checking appearance in mirror." .


###  http://www.owl-ontologies.com/VirtualHome.owl#check_email
ho:check_email rdf:type owl:Class ;
               rdfs:subClassOf ho:Work ;
               rdfs:comment """The class with sequence of actions for checking your mail after you have 
opened it.""" .


###  http://www.owl-ontologies.com/VirtualHome.owl#check_homework
ho:check_homework rdf:type owl:Class ;
                  rdfs:subClassOf ho:Work ;
                  rdfs:comment """The class with sequence of actions for checking homework (either you own 
or anothers person).""" .


###  http://www.owl-ontologies.com/VirtualHome.owl#check_self_in_mirror
ho:check_self_in_mirror rdf:type owl:Class ;
                        rdfs:subClassOf ho:HygieneStyling ;
                        rdfs:comment "The class with sequence of actions for checking your self in the mirror." .


###  http://www.owl-ontologies.com/VirtualHome.owl#chop_vegetables
ho:chop_vegetables rdf:type owl:Class ;
                   rdfs:subClassOf ho:FoodPreparation ;
                   rdfs:comment "Class with sequences on how to cut-chop vegetables in order to prepare dinner, salad, or other kind of food." .


###  http://www.owl-ontologies.com/VirtualHome.owl#clean
ho:clean rdf:type owl:Class ;
         rdfs:subClassOf ho:HouseCleaning ;
         rdfs:comment """Class with general sequences for cleaning, such as clean lamp, bathroom, 
welcome mat.""" .


###  http://www.owl-ontologies.com/VirtualHome.owl#clean_bathroom
ho:clean_bathroom rdf:type owl:Class ;
                  rdfs:subClassOf ho:HouseCleaning ;
                  rdfs:comment """The class with sequence of actions for cleaning the bathroom, the whole 
room.""" .


###  http://www.owl-ontologies.com/VirtualHome.owl#clean_dishes
ho:clean_dishes rdf:type owl:Class ;
                rdfs:subClassOf ho:HouseArrangement ;
                rdfs:comment "The class with sequence of actions for cleaning the dishes." .


###  http://www.owl-ontologies.com/VirtualHome.owl#clean_eggs_from_our_chickens
ho:clean_eggs_from_our_chickens rdf:type owl:Class ;
                                rdfs:subClassOf ho:Other ;
                                rdfs:comment """The class with sequence of actions for cleaning eggs that were produced 
by our chickens.""" .


###  http://www.owl-ontologies.com/VirtualHome.owl#clean_floor
ho:clean_floor rdf:type owl:Class ;
               rdfs:subClassOf ho:HouseCleaning ;
               rdfs:comment "Class with sequences on how to clean the floor." .


###  http://www.owl-ontologies.com/VirtualHome.owl#clean_fridge
ho:clean_fridge rdf:type owl:Class ;
                rdfs:subClassOf ho:HouseCleaning ;
                rdfs:comment """The class with sequence of actions clean the fridge form the inside and 
the outside.""" .


###  http://www.owl-ontologies.com/VirtualHome.owl#clean_glasses
ho:clean_glasses rdf:type owl:Class ;
                 rdfs:subClassOf ho:HouseArrangement ;
                 rdfs:comment "The class with sequence of actions for cleaning watching glasses." .


###  http://www.owl-ontologies.com/VirtualHome.owl#clean_kitchen
ho:clean_kitchen rdf:type owl:Class ;
                 rdfs:subClassOf ho:HouseCleaning ;
                 rdfs:comment """The class with sequence of actions the procedure of cleaning all the 
kitchen.""" .


###  http://www.owl-ontologies.com/VirtualHome.owl#clean_large_jacuzzi_tub
ho:clean_large_jacuzzi_tub rdf:type owl:Class ;
                           rdfs:subClassOf ho:HouseCleaning ;
                           rdfs:comment "The class with sequence of actions for cleaning up a large jacuzzi tab." .


###  http://www.owl-ontologies.com/VirtualHome.owl#clean_mirror
ho:clean_mirror rdf:type owl:Class ;
                rdfs:subClassOf ho:HouseCleaning ;
                rdfs:comment """The class with sequence of actions on how to clean a mirror, no matter 
in which room is in.""" .


###  http://www.owl-ontologies.com/VirtualHome.owl#clean_room
ho:clean_room rdf:type owl:Class ;
              rdfs:subClassOf ho:HouseCleaning ;
              rdfs:comment "The class with sequence of actions on how to clean a room." .


###  http://www.owl-ontologies.com/VirtualHome.owl#clean_screen
ho:clean_screen rdf:type owl:Class ;
                rdfs:subClassOf ho:HouseCleaning ;
                rdfs:comment "The class with sequence of actions for cleaning the screen of the TV, of a computer, or other objects." .


###  http://www.owl-ontologies.com/VirtualHome.owl#clean_sink
ho:clean_sink rdf:type owl:Class ;
              rdfs:subClassOf ho:HouseCleaning ;
              rdfs:comment """Class with sequences for cleaning only the sink, not the surounding, or 
the whole room.""" .


###  http://www.owl-ontologies.com/VirtualHome.owl#clean_toilet
ho:clean_toilet rdf:type owl:Class ;
                rdfs:subClassOf ho:HouseCleaning ;
                rdfs:comment """Class with sequences on how to clean the toilet specifically, not the 
whole bathroom.""" .


###  http://www.owl-ontologies.com/VirtualHome.owl#clear_table
ho:clear_table rdf:type owl:Class ;
               rdfs:subClassOf ho:HouseArrangement ;
               rdfs:comment """The class with sequence of actions for clearing the table after eating 
or claering it because it is dirty.""" .


###  http://www.owl-ontologies.com/VirtualHome.owl#close_curtains
ho:close_curtains rdf:type owl:Class ;
                  rdfs:subClassOf ho:Other ;
                  rdfs:comment "The class with sequence of actions for clossing the curtains, in any room." .


###  http://www.owl-ontologies.com/VirtualHome.owl#close_door
ho:close_door rdf:type owl:Class ;
              rdfs:subClassOf ho:Other ;
              rdfs:comment "The class with sequence of actions for closing the door from any room." .


###  http://www.owl-ontologies.com/VirtualHome.owl#close_dresser_drawer
ho:close_dresser_drawer rdf:type owl:Class ;
                        rdfs:subClassOf ho:Other ;
                        rdfs:comment """The class with sequence of actions for closing dresser drawer, in any 
room.""" .


###  http://www.owl-ontologies.com/VirtualHome.owl#close_shower_curtain
ho:close_shower_curtain rdf:type owl:Class ;
                        rdfs:subClassOf ho:HouseArrangement ;
                        rdfs:comment "The class with sequence of actions for closing shower curtain." .


###  http://www.owl-ontologies.com/VirtualHome.owl#collect_napkin_rings
ho:collect_napkin_rings rdf:type owl:Class ;
                        rdfs:subClassOf ho:HouseArrangement ;
                        rdfs:comment "The class with sequence of actions for collecting napkin rings." .


###  http://www.owl-ontologies.com/VirtualHome.owl#color
ho:color rdf:type owl:Class ;
         rdfs:subClassOf ho:Other ;
         rdfs:comment """The class with sequence of actions for coloring (painting, or painting 
house, etc.).""" .


###  http://www.owl-ontologies.com/VirtualHome.owl#comb_hair
ho:comb_hair rdf:type owl:Class ;
             rdfs:subClassOf ho:HygieneStyling ;
             rdfs:comment "The class with sequence of actions for combing cutting your hair." .


###  http://www.owl-ontologies.com/VirtualHome.owl#come_home
ho:come_home rdf:type owl:Class ;
             rdfs:subClassOf ho:Other ;
             rdfs:comment """The class with sequence of actions for comming home, from wokr, or 
grocery store, etc.""" .


###  http://www.owl-ontologies.com/VirtualHome.owl#come_in_and_leave_home
ho:come_in_and_leave_home rdf:type owl:Class ;
                          rdfs:subClassOf ho:Other ;
                          rdfs:comment """The class with sequence of actions for comming in the house to do 
something, and then get out again.""" .


###  http://www.owl-ontologies.com/VirtualHome.owl#complete_homework
ho:complete_homework rdf:type owl:Class ;
                     rdfs:subClassOf ho:Work ;
                     rdfs:comment "The class with sequence of actions for completing your homework." .


###  http://www.owl-ontologies.com/VirtualHome.owl#complete_school_work
ho:complete_school_work rdf:type owl:Class ;
                        rdfs:subClassOf ho:Work ;
                        rdfs:comment """The class with sequence of actions for completing your school work, this 
is not only homework, could also be getting ready for school.""" .


###  http://www.owl-ontologies.com/VirtualHome.owl#complete_surveys_on_amazon_turk
ho:complete_surveys_on_amazon_turk rdf:type owl:Class ;
                                   rdfs:subClassOf ho:Work ;
                                   rdfs:comment """The class with sequence of actions for completing youe amazon turk 
surveys.""" .


###  http://www.owl-ontologies.com/VirtualHome.owl#compute
ho:compute rdf:type owl:Class ;
           rdfs:subClassOf ho:Other ;
           rdfs:comment "The class with sequence of actions for computing anything." .


###  http://www.owl-ontologies.com/VirtualHome.owl#computer_work
ho:computer_work rdf:type owl:Class ;
                 rdfs:subClassOf ho:Work ;
                 rdfs:comment "The class with sequence of actions to do computer work." .


###  http://www.owl-ontologies.com/VirtualHome.owl#cook_some_food
ho:cook_some_food rdf:type owl:Class ;
                  rdfs:subClassOf ho:FoodPreparation ;
                  rdfs:comment """Class with sequences on how to cook some food prepare the place, the 
order of the ingredience.""" .


###  http://www.owl-ontologies.com/VirtualHome.owl#curled_hair
ho:curled_hair rdf:type owl:Class ;
               rdfs:subClassOf ho:HygieneStyling ;
               rdfs:comment "The class with sequence of actions for making your hair into curle." .


###  http://www.owl-ontologies.com/VirtualHome.owl#cut_bread
ho:cut_bread rdf:type owl:Class ;
             rdfs:subClassOf ho:FoodPreparation ;
             rdfs:comment "The class with sequence of actions for cutting bread." .


###  http://www.owl-ontologies.com/VirtualHome.owl#cut_steak
ho:cut_steak rdf:type owl:Class ;
             rdfs:subClassOf ho:FoodPreparation ;
             rdfs:comment "The class with sequence of actions for cutting the steak." .


###  http://www.owl-ontologies.com/VirtualHome.owl#cut_toenails
ho:cut_toenails rdf:type owl:Class ;
                rdfs:subClassOf ho:HygieneStyling ;
                rdfs:comment "The class with sequence of actions for cutting our toenails." .


###  http://www.owl-ontologies.com/VirtualHome.owl#cut_your_hair
ho:cut_your_hair rdf:type owl:Class ;
                 rdfs:subClassOf ho:HygieneStyling ;
                 rdfs:comment "The class with sequence of actions for cutting you hair." .


###  http://www.owl-ontologies.com/VirtualHome.owl#cutting
ho:cutting rdf:type owl:Class ;
           rdfs:subClassOf ho:Other ;
           rdfs:comment "The class with sequence of actions for cutting any object, in any room." .


###  http://www.owl-ontologies.com/VirtualHome.owl#dance_for_table_as_we_eat
ho:dance_for_table_as_we_eat rdf:type owl:Class ;
                             rdfs:subClassOf ho:EatingDrinking ;
                             rdfs:comment """The class with sequence of actions for dancing for amusement at the 
table as the persons eat.""" .


###  http://www.owl-ontologies.com/VirtualHome.owl#dance_with_kids
ho:dance_with_kids rdf:type owl:Class ;
                   rdfs:subClassOf ho:SocialInteraction ;
                   rdfs:comment "The class with sequence of actions for dancing with kids." .


###  http://www.owl-ontologies.com/VirtualHome.owl#de-wrinkle_sheet
ho:de-wrinkle_sheet rdf:type owl:Class ;
                    rdfs:subClassOf ho:HouseCleaning ;
                    rdfs:comment "The class with sequence of actions for de-wrinkling sheets." .


###  http://www.owl-ontologies.com/VirtualHome.owl#de_wrinkle_sheet
ho:de_wrinkle_sheet rdf:type owl:Class ;
                    rdfs:subClassOf ho:Other ;
                    rdfs:comment """The class with sequence of actions for de-wrinkling the sheet, in any 
room.""" .


###  http://www.owl-ontologies.com/VirtualHome.owl#decorate
ho:decorate rdf:type owl:Class ;
            rdfs:subClassOf ho:HouseArrangement ;
            rdfs:comment """The class with sequence of actions for decoratng any item inside the 
house that can be decorated.""" .


###  http://www.owl-ontologies.com/VirtualHome.owl#decorate_it
ho:decorate_it rdf:type owl:Class ;
               rdfs:subClassOf ho:HouseArrangement ;
               rdfs:comment """The class with sequence of actions for decorating something, after 
getting the token &quot;decorate it&quot;.""" .


###  http://www.owl-ontologies.com/VirtualHome.owl#deficate
ho:deficate rdf:type owl:Class ;
            rdfs:subClassOf ho:HygieneStyling ;
            rdfs:comment "The class with sequence of actions for deficating." .


###  http://www.owl-ontologies.com/VirtualHome.owl#defrost_chicken
ho:defrost_chicken rdf:type owl:Class ;
                   rdfs:subClassOf ho:FoodPreparation ;
                   rdfs:comment "The class with sequence of actions for defrosting chicken." .


###  http://www.owl-ontologies.com/VirtualHome.owl#designing_crafts_with_family
ho:designing_crafts_with_family rdf:type owl:Class ;
                                rdfs:subClassOf ho:Other ;
                                rdfs:comment "The class with sequence of actions for designing crafts with your family." .


###  http://www.owl-ontologies.com/VirtualHome.owl#dining
ho:dining rdf:type owl:Class ;
          rdfs:subClassOf ho:EatingDrinking ;
          rdfs:comment "The class with sequence of actions for dining." .


###  http://www.owl-ontologies.com/VirtualHome.owl#do_an_art_project
ho:do_an_art_project rdf:type owl:Class ;
                     rdfs:subClassOf ho:Other ;
                     rdfs:comment """<p style=\"margin-top: 0\">
      The class with sequence of actions for doing an art project, in any room.
    </p>""" .


###  http://www.owl-ontologies.com/VirtualHome.owl#do_dishes
ho:do_dishes rdf:type owl:Class ;
             rdfs:subClassOf ho:HouseArrangement ;
             rdfs:comment """The class with sequence of actions for doing the dishes, either clean 
them or put them in the cabinet""" .


###  http://www.owl-ontologies.com/VirtualHome.owl#do_facial
ho:do_facial rdf:type owl:Class ;
             rdfs:subClassOf ho:HygieneStyling ;
             rdfs:comment "The class with sequence of actions for doing up a facial." .


###  http://www.owl-ontologies.com/VirtualHome.owl#do_free-style_dance_routine
ho:do_free-style_dance_routine rdf:type owl:Class ;
                               rdfs:subClassOf ho:Other ;
                               rdfs:comment """The class with sequence of actions for doing free style dance routine, 
in any room.""" .


###  http://www.owl-ontologies.com/VirtualHome.owl#do_homework
ho:do_homework rdf:type owl:Class ;
               rdfs:subClassOf ho:Work ;
               rdfs:comment """The class with sequence of actions for writing down your homework (or 
perform other task that will help you finish your homework).""" .


###  http://www.owl-ontologies.com/VirtualHome.owl#do_laundry
ho:do_laundry rdf:type owl:Class ;
              rdfs:subClassOf ho:HouseArrangement ;
              rdfs:comment "The class with sequence of actions for doing the laundry in any room available." .


###  http://www.owl-ontologies.com/VirtualHome.owl#do_nails
ho:do_nails rdf:type owl:Class ;
            rdfs:subClassOf ho:HygieneStyling ;
            rdfs:comment "The class with sequence of actions for doing your nails, hands and feet." .


###  http://www.owl-ontologies.com/VirtualHome.owl#do_taxes
ho:do_taxes rdf:type owl:Class ;
            rdfs:subClassOf ho:Work ;
            rdfs:comment "The class with sequence of actions for doing taxes." .


###  http://www.owl-ontologies.com/VirtualHome.owl#do_work
ho:do_work rdf:type owl:Class ;
           rdfs:subClassOf ho:Work ;
           rdfs:comment "The class with sequence of actions for doing work." .


###  http://www.owl-ontologies.com/VirtualHome.owl#do_work_on_computer
ho:do_work_on_computer rdf:type owl:Class ;
                       rdfs:subClassOf ho:Work ;
                       rdfs:comment """The class with sequence of actions for doing some on the compute, either 
on iths hardware or on the computer itself.""" .


###  http://www.owl-ontologies.com/VirtualHome.owl#do_yoga
ho:do_yoga rdf:type owl:Class ;
           rdfs:subClassOf ho:PhysicalActivity ;
           rdfs:comment "The class with sequence of actions for doing yoga, in any room." .


###  http://www.owl-ontologies.com/VirtualHome.owl#draft_home
ho:draft_home rdf:type owl:Class ;
              rdfs:subClassOf ho:Other ;
              rdfs:comment "The class with sequence of actions for drafting a home, in any room." .


###  http://www.owl-ontologies.com/VirtualHome.owl#draw_picture
ho:draw_picture rdf:type owl:Class ;
                rdfs:subClassOf ho:Other ;
                rdfs:comment """The class with sequence of actions for drawing any picture, either on 
paper or computer.""" .


###  http://www.owl-ontologies.com/VirtualHome.owl#dress_up_and_pretend
ho:dress_up_and_pretend rdf:type owl:Class ;
                        rdfs:subClassOf ho:HygieneStyling ;
                        rdfs:comment """<p style=\"margin-top: 0\">
      The class with sequence of actions for dressing up and pretending.
    </p>""" .


###  http://www.owl-ontologies.com/VirtualHome.owl#dry_hair
ho:dry_hair rdf:type owl:Class ;
            rdfs:subClassOf ho:HygieneStyling ;
            rdfs:comment "The class with sequence of actions for drying your hair." .


###  http://www.owl-ontologies.com/VirtualHome.owl#dry_soap_bottles
ho:dry_soap_bottles rdf:type owl:Class ;
                    rdfs:subClassOf ho:Other ;
                    rdfs:comment "The class with sequence of actions for drying soap bottles, in any room." .


###  http://www.owl-ontologies.com/VirtualHome.owl#dust
ho:dust rdf:type owl:Class ;
        rdfs:subClassOf ho:HouseCleaning ;
        rdfs:comment "Class with sequences about how to dust, different objects." .


###  http://www.owl-ontologies.com/VirtualHome.owl#eat_breakfast
ho:eat_breakfast rdf:type owl:Class ;
                 rdfs:subClassOf ho:FoodPreparation ;
                 rdfs:comment "The class with sequence of actions for eating breakfast in any room." .


###  http://www.owl-ontologies.com/VirtualHome.owl#eat_breaksfast
ho:eat_breaksfast rdf:type owl:Class ;
                  rdfs:subClassOf ho:EatingDrinking ;
                  rdfs:comment "The class with sequence of actions for eating breakfast only." .


###  http://www.owl-ontologies.com/VirtualHome.owl#eat_cereal
ho:eat_cereal rdf:type owl:Class ;
              rdfs:subClassOf ho:EatingDrinking ;
              rdfs:comment "The class with sequence of actions for eating cereals." .


###  http://www.owl-ontologies.com/VirtualHome.owl#eat_cheese
ho:eat_cheese rdf:type owl:Class ;
              rdfs:subClassOf ho:EatingDrinking ;
              rdfs:comment "The class with sequence of actions for eating cheese." .


###  http://www.owl-ontologies.com/VirtualHome.owl#eat_dessert
ho:eat_dessert rdf:type owl:Class ;
               rdfs:subClassOf ho:EatingDrinking ;
               rdfs:comment "The class with sequence of actions for eating dessert in any room." .


###  http://www.owl-ontologies.com/VirtualHome.owl#eat_dinner
ho:eat_dinner rdf:type owl:Class ;
              rdfs:subClassOf ho:EatingDrinking ;
              rdfs:comment "The class with sequence of actions for eating dinner only." .


###  http://www.owl-ontologies.com/VirtualHome.owl#eat_donuts
ho:eat_donuts rdf:type owl:Class ;
              rdfs:subClassOf ho:EatingDrinking ;
              rdfs:comment "The class with sequence of actions for eating donuts." .


###  http://www.owl-ontologies.com/VirtualHome.owl#eat_family_meals
ho:eat_family_meals rdf:type owl:Class ;
                    rdfs:subClassOf ho:EatingDrinking ;
                    rdfs:comment "The class with sequence of actions for eating meals with your family." .


###  http://www.owl-ontologies.com/VirtualHome.owl#eat_ice_cream
ho:eat_ice_cream rdf:type owl:Class ;
                 rdfs:subClassOf ho:EatingDrinking ;
                 rdfs:comment "The class with sequence of actions for eating ice cream in any room." .


###  http://www.owl-ontologies.com/VirtualHome.owl#eat_meals
ho:eat_meals rdf:type owl:Class ;
             rdfs:subClassOf ho:EatingDrinking ;
             rdfs:comment "The class with sequence of actions for eating meals." .


###  http://www.owl-ontologies.com/VirtualHome.owl#eat_on_fancy_china
ho:eat_on_fancy_china rdf:type owl:Class ;
                      rdfs:subClassOf ho:EatingDrinking ;
                      rdfs:comment "The class with sequence of actions for eating at fancy china." .


###  http://www.owl-ontologies.com/VirtualHome.owl#eat_snacks_and_drink_tea
ho:eat_snacks_and_drink_tea rdf:type owl:Class ;
                            rdfs:subClassOf ho:EatingDrinking ;
                            rdfs:comment "The class with sequence of actions for eating snacks and drinking tea." .


###  http://www.owl-ontologies.com/VirtualHome.owl#eat_while_watching_tv
ho:eat_while_watching_tv rdf:type owl:Class ;
                         rdfs:subClassOf ho:EatingDrinking ,
                                         ho:Leisure ;
                         rdfs:comment """The class with sequence of actions for eating something while watching 
TV.""" .


###  http://www.owl-ontologies.com/VirtualHome.owl#empty_dishwasher_and_fill_dishwasher
ho:empty_dishwasher_and_fill_dishwasher rdf:type owl:Class ;
                                        rdfs:subClassOf ho:HouseArrangement ;
                                        rdfs:comment """The class with sequence of actions for emptying dishwasher and fill 
dishwasher, in any room.""" .


###  http://www.owl-ontologies.com/VirtualHome.owl#enjoy_view_out_window
ho:enjoy_view_out_window rdf:type owl:Class ;
                         rdfs:subClassOf ho:Other ;
                         rdfs:comment """The class with sequence of actions for enjoying the view out of the 
window, in any room.""" .


###  http://www.owl-ontologies.com/VirtualHome.owl#enter_home
ho:enter_home rdf:type owl:Class ;
              rdfs:subClassOf ho:Other ;
              rdfs:comment "The class with sequence of actions for entering home." .


###  http://www.owl-ontologies.com/VirtualHome.owl#entertain
ho:entertain rdf:type owl:Class ;
             rdfs:subClassOf ho:SocialInteraction ;
             rdfs:comment """A class with sequences for entertaining your self with activities that 
have to do with other persons.""" .


###  http://www.owl-ontologies.com/VirtualHome.owl#exercise
ho:exercise rdf:type owl:Class ;
            rdfs:subClassOf ho:PhysicalActivity ;
            rdfs:comment "The class with sequence of actions for exercising." .


###  http://www.owl-ontologies.com/VirtualHome.owl#face_washing
ho:face_washing rdf:type owl:Class ;
                rdfs:subClassOf ho:HygieneStyling ;
                rdfs:comment "The class with sequence of actions for washing your face." .


###  http://www.owl-ontologies.com/VirtualHome.owl#family_meetings
ho:family_meetings rdf:type owl:Class ;
                   rdfs:subClassOf ho:SocialInteraction ;
                   rdfs:comment "The class with sequence of actions for family meetings." .


###  http://www.owl-ontologies.com/VirtualHome.owl#fan_magazines_on_coffee_table
ho:fan_magazines_on_coffee_table rdf:type owl:Class ;
                                 rdfs:subClassOf ho:Other ;
                                 rdfs:comment "The class with sequence of actions for fanning magazines on coffee table." .


###  http://www.owl-ontologies.com/VirtualHome.owl#fax_forms_to_doctor
ho:fax_forms_to_doctor rdf:type owl:Class ;
                       rdfs:subClassOf ho:Work ;
                       rdfs:comment "The class with sequence of actions to fax forms to a doctor only." .


###  http://www.owl-ontologies.com/VirtualHome.owl#feed_daughter
ho:feed_daughter rdf:type owl:Class ;
                 rdfs:subClassOf ho:Other ;
                 rdfs:comment "The class with sequence of actions for feeding your daughter." .


###  http://www.owl-ontologies.com/VirtualHome.owl#feed_dog
ho:feed_dog rdf:type owl:Class ;
            rdfs:subClassOf ho:Other ;
            rdfs:comment "The class with sequence of actions for feeding the dog." .


###  http://www.owl-ontologies.com/VirtualHome.owl#feed_me
ho:feed_me rdf:type owl:Class ;
           rdfs:subClassOf ho:Other ;
           rdfs:comment "The class with sequence of actions for feeding the user." .


###  http://www.owl-ontologies.com/VirtualHome.owl#file_documents
ho:file_documents rdf:type owl:Class ;
                  rdfs:subClassOf ho:Work ;
                  rdfs:comment "Class with sequences about how to file the documents." .


###  http://www.owl-ontologies.com/VirtualHome.owl#file_expense_reports
ho:file_expense_reports rdf:type owl:Class ;
                        rdfs:subClassOf ho:Work ;
                        rdfs:comment "The class with sequence of actions for performing file expense reports." .


###  http://www.owl-ontologies.com/VirtualHome.owl#find_dictionary
ho:find_dictionary rdf:type owl:Class ;
                   rdfs:subClassOf ho:Other ;
                   rdfs:comment "The class with sequence of actions for finding the dictionary, in any room search." .


###  http://www.owl-ontologies.com/VirtualHome.owl#fix_bowl_of_cereal
ho:fix_bowl_of_cereal rdf:type owl:Class ;
                      rdfs:subClassOf ho:FoodPreparation ;
                      rdfs:comment """The class with sequence of actions for fixing bowls of cereals (re 
arrange it if it has spilled, or make it look beautiful).""" .


###  http://www.owl-ontologies.com/VirtualHome.owl#fix_broken_toys
ho:fix_broken_toys rdf:type owl:Class ;
                   rdfs:subClassOf ho:Other ;
                   rdfs:comment """The class with sequence of actions for fixing broken toys, any toys in 
any room.""" .


###  http://www.owl-ontologies.com/VirtualHome.owl#fix_sandwhich
ho:fix_sandwhich rdf:type owl:Class ;
                 rdfs:subClassOf ho:FoodPreparation ;
                 rdfs:comment """The class with sequence of actions for fixing sandwhich (make it look 
beautifull, or if it has spilled what it has inside re arragne it).""" .


###  http://www.owl-ontologies.com/VirtualHome.owl#fix_sandwich
ho:fix_sandwich rdf:type owl:Class ;
                rdfs:subClassOf ho:FoodPreparation ;
                rdfs:comment "The class with sequence of actions for fixing a sandwhich." .


###  http://www.owl-ontologies.com/VirtualHome.owl#fix_snack
ho:fix_snack rdf:type owl:Class ;
             rdfs:subClassOf ho:FoodPreparation ;
             rdfs:comment """The class with sequence of actions for fixing a snack (make it look 
beautiful, or re arrange it if ti has beedn torn apart).""" .


###  http://www.owl-ontologies.com/VirtualHome.owl#fluff_pillow
ho:fluff_pillow rdf:type owl:Class ;
                rdfs:subClassOf ho:HouseArrangement ;
                rdfs:comment "The class with sequence of actions for fluffing a pillow, in any room." .


###  http://www.owl-ontologies.com/VirtualHome.owl#fluff_pillows
ho:fluff_pillows rdf:type owl:Class ;
                 rdfs:subClassOf ho:HouseCleaning ;
                 rdfs:comment "The class with sequence of actions for fluffing the pillows." .


###  http://www.owl-ontologies.com/VirtualHome.owl#flush_toilet
ho:flush_toilet rdf:type owl:Class ;
                rdfs:subClassOf ho:HouseCleaning ;
                rdfs:comment "The class with sequence of actions to flush down the toilet." .


###  http://www.owl-ontologies.com/VirtualHome.owl#fold_laundry
ho:fold_laundry rdf:type owl:Class ;
                rdfs:subClassOf ho:HouseArrangement ;
                rdfs:comment """Class with sequences about how to fold the different laundry objects 
(i.e. clothes, or objects that could be considered laundry).""" .


###  http://www.owl-ontologies.com/VirtualHome.owl#gaze_out_window
ho:gaze_out_window rdf:type owl:Class ;
                   rdfs:subClassOf ho:Other ;
                   rdfs:comment "The class with sequence of actions for gazing out the window." .


###  http://www.owl-ontologies.com/VirtualHome.owl#get_dressed
ho:get_dressed rdf:type owl:Class ;
               rdfs:subClassOf ho:HygieneStyling ;
               rdfs:comment """Class with sequences about how to get dressed for getting out, or for 
getting to work.""" .


###  http://www.owl-ontologies.com/VirtualHome.owl#get_drink
ho:get_drink rdf:type owl:Class ;
             rdfs:subClassOf ho:Other ;
             rdfs:comment "The class with sequence of actions for getting a drink, in any room." .


###  http://www.owl-ontologies.com/VirtualHome.owl#get_glass_of_milk
ho:get_glass_of_milk rdf:type owl:Class ;
                     rdfs:subClassOf ho:Other ;
                     rdfs:comment """The class with sequence of actions for getting a glass of milk, from any 
room the milk is in.""" .


###  http://www.owl-ontologies.com/VirtualHome.owl#get_glass_of_water
ho:get_glass_of_water rdf:type owl:Class ;
                      rdfs:subClassOf ho:Other ;
                      rdfs:comment """The class with sequence of actions for getting glass of water, from any 
room that can get water.""" .


###  http://www.owl-ontologies.com/VirtualHome.owl#get_in_way_of_guests_trying_to_leave
ho:get_in_way_of_guests_trying_to_leave rdf:type owl:Class ;
                                        rdfs:subClassOf ho:Other ;
                                        rdfs:comment "The class with sequence of actions for getting in way of guests." .


###  http://www.owl-ontologies.com/VirtualHome.owl#get_mail_ready
ho:get_mail_ready rdf:type owl:Class ;
                  rdfs:subClassOf ho:Work ;
                  rdfs:comment "The class with sequence of actions for getting an email ready to be send." .


###  http://www.owl-ontologies.com/VirtualHome.owl#get_out_dish
ho:get_out_dish rdf:type owl:Class ;
                rdfs:subClassOf ho:Other ;
                rdfs:comment """The class with sequence of actions for getting a dish out, for serving 
in any room.""" .


###  http://www.owl-ontologies.com/VirtualHome.owl#get_ready_for_bed
ho:get_ready_for_bed rdf:type owl:Class ;
                     rdfs:subClassOf ho:BedTimeSleep ;
                     rdfs:comment "\\The class with sequence of actions for getting ready for going to bed." .


###  http://www.owl-ontologies.com/VirtualHome.owl#get_ready_for_day
ho:get_ready_for_day rdf:type owl:Class ;
                     rdfs:subClassOf ho:GettingReady ;
                     rdfs:comment "The class with sequence of actions for getting ready for the day." .


###  http://www.owl-ontologies.com/VirtualHome.owl#get_ready_for_school
ho:get_ready_for_school rdf:type owl:Class ;
                        rdfs:subClassOf ho:GettingReady ;
                        rdfs:comment "The class with sequence of actions for getting ready for school." .


###  http://www.owl-ontologies.com/VirtualHome.owl#get_ready_for_work
ho:get_ready_for_work rdf:type owl:Class ;
                      rdfs:subClassOf ho:GettingReady ;
                      rdfs:comment "The class with sequence of actions for gettinf ready to go to work." .


###  http://www.owl-ontologies.com/VirtualHome.owl#get_ready_to_leave
ho:get_ready_to_leave rdf:type owl:Class ;
                      rdfs:subClassOf ho:GettingReady ;
                      rdfs:comment "The class with sequence of actions for getting ready to leave the house." .


###  http://www.owl-ontologies.com/VirtualHome.owl#get_some_water
ho:get_some_water rdf:type owl:Class ;
                  rdfs:subClassOf ho:Other ;
                  rdfs:comment "The class with sequence of actions for getting some water." .


###  http://www.owl-ontologies.com/VirtualHome.owl#get_something_to_drink
ho:get_something_to_drink rdf:type owl:Class ;
                          rdfs:subClassOf ho:EatingDrinking ;
                          rdfs:comment "The class with sequence of actions for getting something to drink." .


###  http://www.owl-ontologies.com/VirtualHome.owl#get_toilet_paper
ho:get_toilet_paper rdf:type owl:Class ;
                    rdfs:subClassOf ho:Other ;
                    rdfs:comment """The class with sequence of actions for getting toilet paper from any 
room and put it in the toilet.""" .


###  http://www.owl-ontologies.com/VirtualHome.owl#getting__dresses
ho:getting__dresses rdf:type owl:Class ;
                    rdfs:subClassOf ho:Other ;
                    rdfs:comment "The class with sequence of actions for getting dresses." .


###  http://www.owl-ontologies.com/VirtualHome.owl#getting_dressed
ho:getting_dressed rdf:type owl:Class ;
                   rdfs:subClassOf ho:HygieneStyling ;
                   rdfs:comment "The class with sequence of actions for getting dressed." .


###  http://www.owl-ontologies.com/VirtualHome.owl#getting_in_way_of_guest_trying_to_leave
ho:getting_in_way_of_guest_trying_to_leave rdf:type owl:Class ;
                                           rdfs:subClassOf ho:SocialInteraction ;
                                           rdfs:comment """The class with sequence of actions for getting in way of guest trying to 
leave.""" .


###  http://www.owl-ontologies.com/VirtualHome.owl#give_children_bath
ho:give_children_bath rdf:type owl:Class ;
                      rdfs:subClassOf ho:HygieneStyling ,
                                      ho:SocialInteraction ;
                      rdfs:comment "The class with sequence of actions for giving the children a bath." ,
                                   "The class with sequence of actions for giving your children a bath." .


###  http://www.owl-ontologies.com/VirtualHome.owl#give_me_bath
ho:give_me_bath rdf:type owl:Class ;
                rdfs:subClassOf ho:HygieneStyling ;
                rdfs:comment "The class with sequence of actions for giving a bath to the user." .


###  http://www.owl-ontologies.com/VirtualHome.owl#give_milk_to_cat
ho:give_milk_to_cat rdf:type owl:Class ;
                    rdfs:subClassOf ho:Other ;
                    rdfs:comment """The class with sequence of actions for giving milk to the cat, inside 
the house, but in any room.""" .


###  http://www.owl-ontologies.com/VirtualHome.owl#give_your_child_bath
ho:give_your_child_bath rdf:type owl:Class ;
                        rdfs:subClassOf ho:HygieneStyling ;
                        rdfs:comment "The class with sequence of actions for giving you child bath." .


###  http://www.owl-ontologies.com/VirtualHome.owl#go_pee
ho:go_pee rdf:type owl:Class ;
          rdfs:subClassOf ho:HygieneStyling ;
          rdfs:comment "The class with sequence of actions for going to pee." .


###  http://www.owl-ontologies.com/VirtualHome.owl#go_to_bathroom
ho:go_to_bathroom rdf:type owl:Class ;
                  rdfs:subClassOf ho:HygieneStyling ;
                  rdfs:comment "The class with sequence of actions for going to the bathroom." .


###  http://www.owl-ontologies.com/VirtualHome.owl#go_to_bed
ho:go_to_bed rdf:type owl:Class ;
             rdfs:subClassOf ho:BedTimeSleep ;
             rdfs:comment "The class with sequence of actions for going to bed." .


###  http://www.owl-ontologies.com/VirtualHome.owl#go_to_sleep
ho:go_to_sleep rdf:type owl:Class ;
               rdfs:subClassOf ho:BedTimeSleep ;
               rdfs:comment """A class with sequences on how to go to sleep, or get ready to go to 
sleep.""" .


###  http://www.owl-ontologies.com/VirtualHome.owl#go_to_toilet
ho:go_to_toilet rdf:type owl:Class ;
                rdfs:subClassOf ho:HygieneStyling ;
                rdfs:comment "Class with seqeunces on how to go to toilet." .


###  http://www.owl-ontologies.com/VirtualHome.owl#grab_some_juice
ho:grab_some_juice rdf:type owl:Class ;
                   rdfs:subClassOf ho:Other ;
                   rdfs:comment """The class with sequence of actions for grabing some juice, from the 
fridge or elsewhere.""" .


###  http://www.owl-ontologies.com/VirtualHome.owl#grab_things
ho:grab_things rdf:type owl:Class ;
               rdfs:subClassOf ho:Other ;
               rdfs:comment "The class with sequence of actions for grabing things, any object." .


###  http://www.owl-ontologies.com/VirtualHome.owl#grading_papers
ho:grading_papers rdf:type owl:Class ;
                  rdfs:subClassOf ho:Work ;
                  rdfs:comment """The class with sequence of actions for grading some papers (usually for 
school).""" .


###  http://www.owl-ontologies.com/VirtualHome.owl#greet_guests
ho:greet_guests rdf:type owl:Class ;
                rdfs:subClassOf ho:SocialInteraction ;
                rdfs:comment "A class with sequences for greeting guest that have come to your home for visit" .


###  http://www.owl-ontologies.com/VirtualHome.owl#greet_people
ho:greet_people rdf:type owl:Class ;
                rdfs:subClassOf ho:SocialInteraction ;
                rdfs:comment "The class with sequence of actions for greeting people in any room or outside the house." .


###  http://www.owl-ontologies.com/VirtualHome.owl#hair
ho:hair rdf:type owl:Class ;
        rdfs:subClassOf ho:Other ;
        rdfs:comment "The class with sequence of actions for hairing." .


###  http://www.owl-ontologies.com/VirtualHome.owl#hair_dressing
ho:hair_dressing rdf:type owl:Class ;
                 rdfs:subClassOf ho:HygieneStyling ;
                 rdfs:comment "The class with sequence of actions for hair dressing." .


###  http://www.owl-ontologies.com/VirtualHome.owl#hand_washing
ho:hand_washing rdf:type owl:Class ;
                rdfs:subClassOf ho:HygieneStyling ;
                rdfs:comment "The class with sequence of actions for hand washing, in any room." .


###  http://www.owl-ontologies.com/VirtualHome.owl#hang_car_keys
ho:hang_car_keys rdf:type owl:Class ;
                 rdfs:subClassOf ho:Other ;
                 rdfs:comment """The class with sequence of actions for hanging car keys, in any place 
that can be hanged.""" .


###  http://www.owl-ontologies.com/VirtualHome.owl#hang_keys
ho:hang_keys rdf:type owl:Class ;
             rdfs:subClassOf ho:Other ;
             rdfs:comment "The class with sequence of actions for hanging up keys in any room." .


###  http://www.owl-ontologies.com/VirtualHome.owl#hang_out
ho:hang_out rdf:type owl:Class ;
            rdfs:subClassOf ho:Other ;
            rdfs:comment "The class with sequence of actions for hanging out, speending free time in house." .


###  http://www.owl-ontologies.com/VirtualHome.owl#hang_pictures
ho:hang_pictures rdf:type owl:Class ;
                 rdfs:subClassOf ho:HouseArrangement ;
                 rdfs:comment "The class with sequence of actions for hanging out a picture in any room." .


###  http://www.owl-ontologies.com/VirtualHome.owl#hang_up_car_keys
ho:hang_up_car_keys rdf:type owl:Class ;
                    rdfs:subClassOf ho:Other ;
                    rdfs:comment """The class with sequence of actions for hanging up your car keys, in 
every room.""" .


###  http://www.owl-ontologies.com/VirtualHome.owl#hang_up_jacket
ho:hang_up_jacket rdf:type owl:Class ;
                  rdfs:subClassOf ho:Other ;
                  rdfs:comment """A class with sequences on how to hang up your jacket
.""" .


###  http://www.owl-ontologies.com/VirtualHome.owl#hang_up_poster
ho:hang_up_poster rdf:type owl:Class ;
                  rdfs:subClassOf ho:HouseArrangement ;
                  rdfs:comment "The class with sequence of actions for hanging up the poster in any room." .


###  http://www.owl-ontologies.com/VirtualHome.owl#hang_with_friend
ho:hang_with_friend rdf:type owl:Class ;
                    rdfs:subClassOf ho:SocialInteraction ;
                    rdfs:comment """The class with sequence of actions for hanging with your friend inside 
the house.""" .


###  http://www.owl-ontologies.com/VirtualHome.owl#hang_with_friends
ho:hang_with_friends rdf:type owl:Class ;
                     rdfs:subClassOf ho:Other ;
                     rdfs:comment "The class with sequence of actions for hanging with friends." .


###  http://www.owl-ontologies.com/VirtualHome.owl#have_conversation_with_boyfriend
ho:have_conversation_with_boyfriend rdf:type owl:Class ;
                                    rdfs:subClassOf ho:SocialInteraction ;
                                    rdfs:comment """The class with sequence of actions for having conversation with your 
boyfriend.""" .


###  http://www.owl-ontologies.com/VirtualHome.owl#have_dinner
ho:have_dinner rdf:type owl:Class ;
               rdfs:subClassOf ho:EatingDrinking ;
               rdfs:comment "The class with sequence of actions for having dinner." .


###  http://www.owl-ontologies.com/VirtualHome.owl#have_ice_coffee
ho:have_ice_coffee rdf:type owl:Class ;
                   rdfs:subClassOf ho:EatingDrinking ;
                   rdfs:comment "The class with sequence of actions for drinking ice coffee in any room." .


###  http://www.owl-ontologies.com/VirtualHome.owl#have_party
ho:have_party rdf:type owl:Class ;
              rdfs:subClassOf ho:SocialInteraction ;
              rdfs:comment "The class with sequence of actions for having a party inside the house." .


###  http://www.owl-ontologies.com/VirtualHome.owl#have_quality_family_time
ho:have_quality_family_time rdf:type owl:Class ;
                            rdfs:subClassOf ho:SocialInteraction ;
                            rdfs:comment "The class with sequence of actions for having qualtiy family time, no matter the members if the family." .


###  http://www.owl-ontologies.com/VirtualHome.owl#have_snack
ho:have_snack rdf:type owl:Class ;
              rdfs:subClassOf ho:EatingDrinking ;
              rdfs:comment """The class with sequence of actions for having a snack at any time of the 
day.""" .


###  http://www.owl-ontologies.com/VirtualHome.owl#have_tea_party
ho:have_tea_party rdf:type owl:Class ;
                  rdfs:subClassOf ho:SocialInteraction ;
                  rdfs:comment "The class with sequence of actions for having a tea party." .


###  http://www.owl-ontologies.com/VirtualHome.owl#help_kids_with_homework
ho:help_kids_with_homework rdf:type owl:Class ;
                           rdfs:subClassOf ho:SocialInteraction ;
                           rdfs:comment "The class with sequence of actions for helping kids with their homework." .


###  http://www.owl-ontologies.com/VirtualHome.owl#help_organize_files
ho:help_organize_files rdf:type owl:Class ;
                       rdfs:subClassOf ho:Other ;
                       rdfs:comment """The class with sequence of actions for helping organize the files, in 
any order.""" .


###  http://www.owl-ontologies.com/VirtualHome.owl#help_with_quiz_shows
ho:help_with_quiz_shows rdf:type owl:Class ;
                        rdfs:subClassOf ho:Other ;
                        rdfs:comment """The class with sequence of actions for helping with quiz shows, any 
person.""" .


###  http://www.owl-ontologies.com/VirtualHome.owl#hide
ho:hide rdf:type owl:Class ;
        rdfs:subClassOf ho:Other ;
        rdfs:comment "The class with sequence of actions for hiding in any room." .


###  http://www.owl-ontologies.com/VirtualHome.owl#hold_coats_and_umbrellas
ho:hold_coats_and_umbrellas rdf:type owl:Class ;
                            rdfs:subClassOf ho:HouseArrangement ;
                            rdfs:comment """The class with sequence of actions for holding your coat (or coats) and 
an umbrella.""" .


###  http://www.owl-ontologies.com/VirtualHome.owl#homework
ho:homework rdf:type owl:Class ;
            rdfs:subClassOf ho:Work ;
            rdfs:comment "The class with sequence of actions for actions for getting ready for homework." .


###  http://www.owl-ontologies.com/VirtualHome.owl#ignore_people
ho:ignore_people rdf:type owl:Class ;
                 rdfs:subClassOf ho:SocialInteraction ;
                 rdfs:comment "The class with sequence of actions for ignoring the people inside the room." .


###  http://www.owl-ontologies.com/VirtualHome.owl#in_living_room_i_eat_dinner
ho:in_living_room_i_eat_dinner rdf:type owl:Class ;
                               rdfs:subClassOf ho:Leisure ;
                               rdfs:comment "The class with sequence of actions for eating dinner in living room." .


###  http://www.owl-ontologies.com/VirtualHome.owl#iron_shirt
ho:iron_shirt rdf:type owl:Class ;
              rdfs:subClassOf ho:HouseArrangement ;
              rdfs:comment """The class with sequence of actions for ironing a shirt in any place or 
room.""" .


###  http://www.owl-ontologies.com/VirtualHome.owl#juggling
ho:juggling rdf:type owl:Class ;
            rdfs:subClassOf ho:Leisure ;
            rdfs:comment """The class with sequence of actions for juggling (whatever object can 
fly).""" .


###  http://www.owl-ontologies.com/VirtualHome.owl#keep_an_eye_on_stove_as_something_is_cooking
ho:keep_an_eye_on_stove_as_something_is_cooking rdf:type owl:Class ;
                                                rdfs:subClassOf ho:FoodPreparation ;
                                                rdfs:comment """The class with sequence of actions for keeping an eye on stove as 
somehting is cooking.""" .


###  http://www.owl-ontologies.com/VirtualHome.owl#keep_cats_inside_while_door_is_open
ho:keep_cats_inside_while_door_is_open rdf:type owl:Class ;
                                       rdfs:subClassOf ho:Other ;
                                       rdfs:comment """The class with sequence of actions for trying to keep cats inside while 
door is open.""" .


###  http://www.owl-ontologies.com/VirtualHome.owl#keep_cats_out_of_room
ho:keep_cats_out_of_room rdf:type owl:Class ;
                         rdfs:subClassOf ho:SocialInteraction ;
                         rdfs:comment """The class with sequence of actions for keepin the cats out of room
, any room.""" .


###  http://www.owl-ontologies.com/VirtualHome.owl#lay_down_on_floor_and_say_im_rug
ho:lay_down_on_floor_and_say_im_rug rdf:type owl:Class ;
                                    rdfs:subClassOf ho:Other ;
                                    rdfs:comment """The class with sequence of actions for laying down on floor in any room 
and say, I am rug.""" .


###  http://www.owl-ontologies.com/VirtualHome.owl#lay_tablecloth
ho:lay_tablecloth rdf:type owl:Class ;
                  rdfs:subClassOf ho:HouseArrangement ;
                  rdfs:comment """The class with sequence of actions for laying the tablecoth on the 
table, in any room.""" .


###  http://www.owl-ontologies.com/VirtualHome.owl#leave_home
ho:leave_home rdf:type owl:Class ;
              rdfs:subClassOf ho:Other ;
              rdfs:comment "The class with sequence of actions for leaving home." .


###  http://www.owl-ontologies.com/VirtualHome.owl#let_baby_learn_how_to_walk
ho:let_baby_learn_how_to_walk rdf:type owl:Class ;
                              rdfs:subClassOf ho:Other ;
                              rdfs:comment "The class with sequence of actions for letting the baby learn how to walk." .


###  http://www.owl-ontologies.com/VirtualHome.owl#let_bay_learn_how_to_walk
ho:let_bay_learn_how_to_walk rdf:type owl:Class ;
                             rdfs:subClassOf ho:SocialInteraction ;
                             rdfs:comment """The class with sequence of actions for letting your child or baby to 
learn how to walk.""" .


###  http://www.owl-ontologies.com/VirtualHome.owl#light_candle
ho:light_candle rdf:type owl:Class ;
                rdfs:subClassOf ho:Other ;
                rdfs:comment "The class with sequence of actions for lighting up a candle in any room." .


###  http://www.owl-ontologies.com/VirtualHome.owl#light_candles
ho:light_candles rdf:type owl:Class ;
                 rdfs:subClassOf ho:HouseArrangement ;
                 rdfs:comment "The class with sequence of actions for lighting up the candles." .


###  http://www.owl-ontologies.com/VirtualHome.owl#listen_to_music
ho:listen_to_music rdf:type owl:Class ;
                   rdfs:subClassOf ho:Leisure ;
                   rdfs:comment "The class which contains sequences for listening to music." .


###  http://www.owl-ontologies.com/VirtualHome.owl#load_dishwasher
ho:load_dishwasher rdf:type owl:Class ;
                   rdfs:subClassOf ho:HouseArrangement ;
                   rdfs:comment """The class with sequence of actions for laoding up the dishwasher
.""" .


###  http://www.owl-ontologies.com/VirtualHome.owl#lock_door
ho:lock_door rdf:type owl:Class ;
             rdfs:subClassOf ho:Other ;
             rdfs:comment "The class with sequence of actions for locking the door in any room." .


###  http://www.owl-ontologies.com/VirtualHome.owl#look_at_mirror
ho:look_at_mirror rdf:type owl:Class ;
                  rdfs:subClassOf ho:Other ;
                  rdfs:comment "The class with sequence of actions for looking at the mirror in any room." .


###  http://www.owl-ontologies.com/VirtualHome.owl#look_at_painting
ho:look_at_painting rdf:type owl:Class ;
                    rdfs:subClassOf ho:Other ;
                    rdfs:comment "The class with sequence of actions for looki g at painting in any room." .


###  http://www.owl-ontologies.com/VirtualHome.owl#look_in_refrigerator
ho:look_in_refrigerator rdf:type owl:Class ;
                        rdfs:subClassOf ho:Other ;
                        rdfs:comment """The class with sequence of actions for looking in refrigerator for any 
reason.""" .


###  http://www.owl-ontologies.com/VirtualHome.owl#look_out_window
ho:look_out_window rdf:type owl:Class ;
                   rdfs:subClassOf ho:Other ;
                   rdfs:comment """The class with sequence of actions for looking out the window, in any 
room.""" .


###  http://www.owl-ontologies.com/VirtualHome.owl#mail_signed_letter_to_customer
ho:mail_signed_letter_to_customer rdf:type owl:Class ;
                                  rdfs:subClassOf ho:Work ;
                                  rdfs:comment """The class with sequence of actions read-send a mail that contains a 
signed letter for the customer.""" .


###  http://www.owl-ontologies.com/VirtualHome.owl#make__cookies
ho:make__cookies rdf:type owl:Class ;
                 rdfs:subClassOf ho:FoodPreparation ;
                 rdfs:comment "The class with sequence of actions for making cookies in any room." .


###  http://www.owl-ontologies.com/VirtualHome.owl#make_banana_bread
ho:make_banana_bread rdf:type owl:Class ;
                     rdfs:subClassOf ho:FoodPreparation ;
                     rdfs:comment """The class with sequence of actions for making a bread that contains 
banana.""" .


###  http://www.owl-ontologies.com/VirtualHome.owl#make_bed
ho:make_bed rdf:type owl:Class ;
            rdfs:subClassOf ho:HouseArrangement ;
            rdfs:comment """Class with sequences about how to make you own bed, under different 
circumstances.""" .


###  http://www.owl-ontologies.com/VirtualHome.owl#make_cereal
ho:make_cereal rdf:type owl:Class ;
               rdfs:subClassOf ho:FoodPreparation ;
               rdfs:comment "The class with sequence of actions for making cereals." .


###  http://www.owl-ontologies.com/VirtualHome.owl#make_childs_bed
ho:make_childs_bed rdf:type owl:Class ;
                   rdfs:subClassOf ho:HouseArrangement ;
                   rdfs:comment "The class with sequence of actions for making the childs bed in any room." .


###  http://www.owl-ontologies.com/VirtualHome.owl#make_coffee
ho:make_coffee rdf:type owl:Class ;
               rdfs:subClassOf ho:FoodPreparation ;
               rdfs:comment "Class with sequences on how to make coffee with different methods, and different steps." .


###  http://www.owl-ontologies.com/VirtualHome.owl#make_drink
ho:make_drink rdf:type owl:Class ;
              rdfs:subClassOf ho:FoodPreparation ;
              rdfs:comment "The class with sequence of actions for making a drink." .


###  http://www.owl-ontologies.com/VirtualHome.owl#make_eggs
ho:make_eggs rdf:type owl:Class ;
             rdfs:subClassOf ho:FoodPreparation ;
             rdfs:comment "The class with sequence of actions for making eggs." .


###  http://www.owl-ontologies.com/VirtualHome.owl#make_ice_in_ice_trays_for_freezer
ho:make_ice_in_ice_trays_for_freezer rdf:type owl:Class ;
                                     rdfs:subClassOf ho:FoodPreparation ;
                                     rdfs:comment """The class with sequence of actions for making ice in ice trays fo 
freezer.""" .


###  http://www.owl-ontologies.com/VirtualHome.owl#make_iced_coffee
ho:make_iced_coffee rdf:type owl:Class ;
                    rdfs:subClassOf ho:FoodPreparation ;
                    rdfs:comment "The class with sequence of actions for making iced coffee only." .


###  http://www.owl-ontologies.com/VirtualHome.owl#make_jello
ho:make_jello rdf:type owl:Class ;
              rdfs:subClassOf ho:FoodPreparation ;
              rdfs:comment "The class with sequence of actions for making jello." .


###  http://www.owl-ontologies.com/VirtualHome.owl#make_kids_bed
ho:make_kids_bed rdf:type owl:Class ;
                 rdfs:subClassOf ho:HouseArrangement ;
                 rdfs:comment "The class with sequence of actions for making the kids bed, in any room." .


###  http://www.owl-ontologies.com/VirtualHome.owl#make_peanut_butter_sandwhich
ho:make_peanut_butter_sandwhich rdf:type owl:Class ;
                                rdfs:subClassOf ho:FoodPreparation ;
                                rdfs:comment "The class with sequence of actions for making peanut butter sandwhich." .


###  http://www.owl-ontologies.com/VirtualHome.owl#make_peanut_butter_sandwich
ho:make_peanut_butter_sandwich rdf:type owl:Class ;
                               rdfs:subClassOf ho:FoodPreparation ;
                               rdfs:comment "The class with sequence of actions for making peanut butter sandwhich." .


###  http://www.owl-ontologies.com/VirtualHome.owl#make_phone_call
ho:make_phone_call rdf:type owl:Class ;
                   rdfs:subClassOf ho:SocialInteraction ;
                   rdfs:comment "The class with sequence of actions for making a phone call, form cell phone or home phone." .


###  http://www.owl-ontologies.com/VirtualHome.owl#make_place_cards
ho:make_place_cards rdf:type owl:Class ;
                    rdfs:subClassOf ho:Other ;
                    rdfs:comment "The class with sequence of actions for making place cards." .


###  http://www.owl-ontologies.com/VirtualHome.owl#make_popcorn
ho:make_popcorn rdf:type owl:Class ;
                rdfs:subClassOf ho:FoodPreparation ;
                rdfs:comment """The class with sequence of actions for making popcorn, in what ever mean 
can cook popcorn.""" .


###  http://www.owl-ontologies.com/VirtualHome.owl#make_sandwich
ho:make_sandwich rdf:type owl:Class ;
                 rdfs:subClassOf ho:FoodPreparation ;
                 rdfs:comment "The class with sequence of actions for making sandwich." .


###  http://www.owl-ontologies.com/VirtualHome.owl#make_sandwitch
ho:make_sandwitch rdf:type owl:Class ;
                  rdfs:subClassOf ho:FoodPreparation ;
                  rdfs:comment "The class with sequence of actions for making a sandwitch." .


###  http://www.owl-ontologies.com/VirtualHome.owl#make_several_copies_on_printer
ho:make_several_copies_on_printer rdf:type owl:Class ;
                                  rdfs:subClassOf ho:Work ;
                                  rdfs:comment """The class with sequence of actions to make several copies on the 
printer, the file does not matter in this case.""" .


###  http://www.owl-ontologies.com/VirtualHome.owl#make_tea
ho:make_tea rdf:type owl:Class ;
            rdfs:subClassOf ho:FoodPreparation ;
            rdfs:comment "The class with sequence of actions for making tea." .


###  http://www.owl-ontologies.com/VirtualHome.owl#make_toast
ho:make_toast rdf:type owl:Class ;
              rdfs:subClassOf ho:FoodPreparation ;
              rdfs:comment """The class with sequence of actions for making your own toast, or for 
someone else.""" .


###  http://www.owl-ontologies.com/VirtualHome.owl#make_tomato_sauce
ho:make_tomato_sauce rdf:type owl:Class ;
                     rdfs:subClassOf ho:FoodPreparation ;
                     rdfs:comment """The class with sequence of actions for making tomatoes sauce, in any 
room.""" .


###  http://www.owl-ontologies.com/VirtualHome.owl#make_tutu
ho:make_tutu rdf:type owl:Class ;
             rdfs:subClassOf ho:Other ;
             rdfs:comment "The class with sequence of actions for making tutu, inside the house." .


###  http://www.owl-ontologies.com/VirtualHome.owl#make_up_bed_for_guest_on_couch
ho:make_up_bed_for_guest_on_couch rdf:type owl:Class ;
                                  rdfs:subClassOf ho:HouseArrangement ;
                                  rdfs:comment """The class with sequence of actions for making up bed for guest on couch, 
wherever the couch is in the house.""" .


###  http://www.owl-ontologies.com/VirtualHome.owl#manage_documents
ho:manage_documents rdf:type owl:Class ;
                    rdfs:subClassOf ho:Work ;
                    rdfs:comment "The class with sequence of actions on how to manage your documents." .


###  http://www.owl-ontologies.com/VirtualHome.owl#manage_emails
ho:manage_emails rdf:type owl:Class ;
                 rdfs:subClassOf ho:Work ;
                 rdfs:comment """The class with sequence of actions for managing your emails (sorting, or 
merging the different files with emails).""" .


###  http://www.owl-ontologies.com/VirtualHome.owl#massage
ho:massage rdf:type owl:Class ;
           rdfs:subClassOf ho:SocialInteraction ;
           rdfs:comment "The class with sequence of actions for doing massage in any room." .


###  http://www.owl-ontologies.com/VirtualHome.owl#meeting
ho:meeting rdf:type owl:Class ;
           rdfs:subClassOf ho:SocialInteraction ;
           rdfs:comment """The class with sequence of actions for meeting , no matter the purpose 
of meeting.""" .


###  http://www.owl-ontologies.com/VirtualHome.owl#mop
ho:mop rdf:type owl:Class ;
       rdfs:subClassOf ho:HouseCleaning ;
       rdfs:comment "The class with sequence of actions taking up the mop and cleaning." .


###  http://www.owl-ontologies.com/VirtualHome.owl#mop_floor
ho:mop_floor rdf:type owl:Class ;
             rdfs:subClassOf ho:HouseCleaning ;
             rdfs:comment "The class with sequence of actions for mopping the floor." .


###  http://www.owl-ontologies.com/VirtualHome.owl#movie
ho:movie rdf:type owl:Class ;
         rdfs:subClassOf ho:Leisure ;
         rdfs:comment """The class with sequence of actions for watching a movie, either at TV or 
your Laptop.""" .


###  http://www.owl-ontologies.com/VirtualHome.owl#oil_dining_room
ho:oil_dining_room rdf:type owl:Class ;
                   rdfs:subClassOf ho:HouseCleaning ;
                   rdfs:comment "The class with sequence of actions for oiling dining room." .


###  http://www.owl-ontologies.com/VirtualHome.owl#open_bathroom_window
ho:open_bathroom_window rdf:type owl:Class ;
                        rdfs:subClassOf ho:Other ;
                        rdfs:comment "The class with sequence of actions for opening bathroom window." .


###  http://www.owl-ontologies.com/VirtualHome.owl#open_curtains
ho:open_curtains rdf:type owl:Class ;
                 rdfs:subClassOf ho:Other ;
                 rdfs:comment """The class with sequence of actions for opening up the curtains, from any 
room inside the house.""" .


###  http://www.owl-ontologies.com/VirtualHome.owl#open_door
ho:open_door rdf:type owl:Class ;
             rdfs:subClassOf ho:Other ;
             rdfs:comment """The class with sequence of actions for opening the door, either from the 
main entrance or door of a room.""" .


###  http://www.owl-ontologies.com/VirtualHome.owl#open_door_and_great_guests
ho:open_door_and_great_guests rdf:type owl:Class ;
                              rdfs:subClassOf ho:SocialInteraction ;
                              rdfs:comment "The class with sequence of actions for opening the door and greeting guests." .


###  http://www.owl-ontologies.com/VirtualHome.owl#open_front_door
ho:open_front_door rdf:type owl:Class ;
                   rdfs:subClassOf ho:Other ;
                   rdfs:comment """The class with sequence of actions for opening front door (main entrance 
door).""" .


###  http://www.owl-ontologies.com/VirtualHome.owl#open_window
ho:open_window rdf:type owl:Class ;
               rdfs:subClassOf ho:Other ;
               rdfs:comment "The class with sequence of actions for opening a window in any room." .


###  http://www.owl-ontologies.com/VirtualHome.owl#order_office_suplies
ho:order_office_suplies rdf:type owl:Class ;
                        rdfs:subClassOf ho:Work ;
                        rdfs:comment """The class with sequence of actions for ordering office suplies, such as 
papers, writing material, and more.""" .


###  http://www.owl-ontologies.com/VirtualHome.owl#organise_paperwork
ho:organise_paperwork rdf:type owl:Class ;
                      rdfs:subClassOf ho:Work ;
                      rdfs:comment "The class with sequence of actions for organizing paperwork." .


###  http://www.owl-ontologies.com/VirtualHome.owl#organize
ho:organize rdf:type owl:Class ;
            rdfs:subClassOf ho:Other ;
            rdfs:comment """The class with sequence of actions for organizing your work, your 
clothes, etc.""" .


###  http://www.owl-ontologies.com/VirtualHome.owl#organize_cabinet
ho:organize_cabinet rdf:type owl:Class ;
                    rdfs:subClassOf ho:HouseArrangement ;
                    rdfs:comment """The class with sequence of actions for organizing the objects insde the 
cabinet.""" .


###  http://www.owl-ontologies.com/VirtualHome.owl#organize_closet
ho:organize_closet rdf:type owl:Class ;
                   rdfs:subClassOf ho:HouseCleaning ;
                   rdfs:comment "The class with sequence of actions for organizing the closet." .


###  http://www.owl-ontologies.com/VirtualHome.owl#organize_desk
ho:organize_desk rdf:type owl:Class ;
                 rdfs:subClassOf ho:HouseArrangement ;
                 rdfs:comment """The class with sequence of actions for organizing the desk place, 
sorting items, pick up items.""" .


###  http://www.owl-ontologies.com/VirtualHome.owl#organize_files
ho:organize_files rdf:type owl:Class ;
                  rdfs:subClassOf ho:Other ;
                  rdfs:comment "The class with sequence of actions for organizing files, in anu order desired." .


###  http://www.owl-ontologies.com/VirtualHome.owl#organize_panrty
ho:organize_panrty rdf:type owl:Class ;
                   rdfs:subClassOf ho:HouseArrangement ;
                   rdfs:comment """The class with sequence of actions for organizing party, by using your 
phone or computer.""" .


###  http://www.owl-ontologies.com/VirtualHome.owl#organize_paperwork
ho:organize_paperwork rdf:type owl:Class ;
                      rdfs:subClassOf ho:Work ;
                      rdfs:comment "The class with sequence of actions for organizing your paper work." .


###  http://www.owl-ontologies.com/VirtualHome.owl#pack_lunch
ho:pack_lunch rdf:type owl:Class ;
              rdfs:subClassOf ho:Other ;
              rdfs:comment "The class with sequence of actions for packing up lunch, and go anywhere." .


###  http://www.owl-ontologies.com/VirtualHome.owl#paint_ceiling
ho:paint_ceiling rdf:type owl:Class ;
                 rdfs:subClassOf ho:HouseArrangement ;
                 rdfs:comment "The class with sequence of actions for painting the ceiling only." .


###  http://www.owl-ontologies.com/VirtualHome.owl#paint_nails
ho:paint_nails rdf:type owl:Class ;
               rdfs:subClassOf ho:HygieneStyling ;
               rdfs:comment "The class with sequence of actions for painting your own nails." .


###  http://www.owl-ontologies.com/VirtualHome.owl#pay_bills
ho:pay_bills rdf:type owl:Class ;
             rdfs:subClassOf ho:Work ;
             rdfs:comment "Class that contains sequences about how to pay bills." .


###  http://www.owl-ontologies.com/VirtualHome.owl#pee
ho:pee rdf:type owl:Class ;
       rdfs:subClassOf ho:HygieneStyling ;
       rdfs:comment "The class with sequence of actions for peeing." .


###  http://www.owl-ontologies.com/VirtualHome.owl#peel_kiwi
ho:peel_kiwi rdf:type owl:Class ;
             rdfs:subClassOf ho:FoodPreparation ;
             rdfs:comment "The class with sequence of actions for pelling the kiwi fruit." .


###  http://www.owl-ontologies.com/VirtualHome.owl#peel_potatoes
ho:peel_potatoes rdf:type owl:Class ;
                 rdfs:subClassOf ho:FoodPreparation ;
                 rdfs:comment "The class with sequence of actions for peeling potatoes in any room." .


###  http://www.owl-ontologies.com/VirtualHome.owl#pet_cat
ho:pet_cat rdf:type owl:Class ;
           rdfs:subClassOf ho:SocialInteraction ;
           rdfs:comment "A class with sequeces on how to pet your cat.." .


###  http://www.owl-ontologies.com/VirtualHome.owl#pet_dog
ho:pet_dog rdf:type owl:Class ;
           rdfs:subClassOf ho:Other ;
           rdfs:comment "The class with sequence of actions for petting your dog." .


###  http://www.owl-ontologies.com/VirtualHome.owl#physical_therapy
ho:physical_therapy rdf:type owl:Class ;
                    rdfs:subClassOf ho:PhysicalActivity ;
                    rdfs:comment "The class with sequence of actions for doing physical therapy." .


###  http://www.owl-ontologies.com/VirtualHome.owl#pick_toys
ho:pick_toys rdf:type owl:Class ;
             rdfs:subClassOf ho:HouseArrangement ;
             rdfs:comment """The class with sequence of actions for picking up toys that were thrown 
away.""" .


###  http://www.owl-ontologies.com/VirtualHome.owl#pick_up
ho:pick_up rdf:type owl:Class ;
           rdfs:subClassOf ho:Other ;
           rdfs:comment """The class with sequence of actions for picking up any object, in any 
room.""" .


###  http://www.owl-ontologies.com/VirtualHome.owl#pick_up_all_trash
ho:pick_up_all_trash rdf:type owl:Class ;
                     rdfs:subClassOf ho:Other ;
                     rdfs:comment """The class with sequence of actions for picking up all trash from the 
floor, or any other place.""" .


###  http://www.owl-ontologies.com/VirtualHome.owl#pick_up_cat_hair
ho:pick_up_cat_hair rdf:type owl:Class ;
                    rdfs:subClassOf ho:HouseCleaning ;
                    rdfs:comment "The class with sequence of actions picking up the cat hair from the various furniture and the floor." .


###  http://www.owl-ontologies.com/VirtualHome.owl#pick_up_dIshes
ho:pick_up_dIshes rdf:type owl:Class ;
                  rdfs:subClassOf ho:HouseArrangement ;
                  rdfs:comment "The class with sequence of actions for picking up the dishes, from any room." .


###  http://www.owl-ontologies.com/VirtualHome.owl#pick_up_dirty_dishes
ho:pick_up_dirty_dishes rdf:type owl:Class ;
                        rdfs:subClassOf ho:HouseArrangement ;
                        rdfs:comment """The class with sequence of actions for picking up dirty dishes, in any 
room.""" .


###  http://www.owl-ontologies.com/VirtualHome.owl#pick_up_dishes
ho:pick_up_dishes rdf:type owl:Class ;
                  rdfs:subClassOf ho:Other ;
                  rdfs:comment "The class with sequence of actions for picking up the dishes." .


###  http://www.owl-ontologies.com/VirtualHome.owl#pick_up_obvious_trash
ho:pick_up_obvious_trash rdf:type owl:Class ;
                         rdfs:subClassOf ho:Other ;
                         rdfs:comment """The class with sequence of actions for picking up objects that are 
obiously trash.""" .


###  http://www.owl-ontologies.com/VirtualHome.owl#pick_up_phone
ho:pick_up_phone rdf:type owl:Class ;
                 rdfs:subClassOf ho:Other ;
                 rdfs:comment """A class with sequences on how to answer the phone, from different rooms, 
and in different scenaria sucks as holding something in hands, etc.""" .


###  http://www.owl-ontologies.com/VirtualHome.owl#pick_up_spare_change_on_dresser
ho:pick_up_spare_change_on_dresser rdf:type owl:Class ;
                                   rdfs:subClassOf ho:Other ;
                                   rdfs:comment "The class with sequence of actions for picking up sparse change on dresser, in any room." .


###  http://www.owl-ontologies.com/VirtualHome.owl#pick_up_toys
ho:pick_up_toys rdf:type owl:Class ;
                rdfs:subClassOf ho:Other ;
                rdfs:comment """A class with sequences on to pick up the toys left behind by other 
individuals.""" .


###  http://www.owl-ontologies.com/VirtualHome.owl#place_bathmat
ho:place_bathmat rdf:type owl:Class ;
                 rdfs:subClassOf ho:HouseArrangement ;
                 rdfs:comment "The class with sequence of actions for placing bathmat in the bathroom." .


###  http://www.owl-ontologies.com/VirtualHome.owl#place_centerpiece
ho:place_centerpiece rdf:type owl:Class ;
                     rdfs:subClassOf ho:HouseArrangement ;
                     rdfs:comment "The class with sequence of actions for placing centerpiece." .


###  http://www.owl-ontologies.com/VirtualHome.owl#place_table
ho:place_table rdf:type owl:Class ;
               rdfs:subClassOf ho:HouseArrangement ;
               rdfs:comment "The class with sequence of actions for placing the table in any room." .


###  http://www.owl-ontologies.com/VirtualHome.owl#play_fetch_with_dog
ho:play_fetch_with_dog rdf:type owl:Class ;
                       rdfs:subClassOf ho:SocialInteraction ;
                       rdfs:comment "The class with sequence of actions for playing fetch with a dog." .


###  http://www.owl-ontologies.com/VirtualHome.owl#play_games
ho:play_games rdf:type owl:Class ;
              rdfs:subClassOf ho:Leisure ;
              rdfs:comment "The sequence of actions about how to paly games." .


###  http://www.owl-ontologies.com/VirtualHome.owl#play_guitar
ho:play_guitar rdf:type owl:Class ;
               rdfs:subClassOf ho:Leisure ;
               rdfs:comment """The class with sequence of actions for playing with the guitar (electric 
or normal).""" .


###  http://www.owl-ontologies.com/VirtualHome.owl#play_musical_chairs
ho:play_musical_chairs rdf:type owl:Class ;
                       rdfs:subClassOf ho:Leisure ;
                       rdfs:comment "The class with sequence of actions for playing musical chairs, (with no respect to the environment)." .


###  http://www.owl-ontologies.com/VirtualHome.owl#play_on_laptop
ho:play_on_laptop rdf:type owl:Class ;
                  rdfs:subClassOf ho:Leisure ;
                  rdfs:comment "The class with sequence of actions for palying games or have fyn while at your computer." .


###  http://www.owl-ontologies.com/VirtualHome.owl#play_piano
ho:play_piano rdf:type owl:Class ;
              rdfs:subClassOf ho:Leisure ;
              rdfs:comment "The class with sequence of actions for playing your piano." .


###  http://www.owl-ontologies.com/VirtualHome.owl#play_with_barbies
ho:play_with_barbies rdf:type owl:Class ;
                     rdfs:subClassOf ho:Leisure ;
                     rdfs:comment """<p style=\"margin-top: 0\">
      The class with sequence of actions for palying with barbie dolls.
    </p>""" .


###  http://www.owl-ontologies.com/VirtualHome.owl#play_with_toys
ho:play_with_toys rdf:type owl:Class ;
                  rdfs:subClassOf ho:Other ;
                  rdfs:comment "The class with sequence of actions for playing with toys, in any room." .


###  http://www.owl-ontologies.com/VirtualHome.owl#playing_video_game
ho:playing_video_game rdf:type owl:Class ;
                      rdfs:subClassOf ho:Leisure ;
                      rdfs:comment """The class with sequence of actions either at a console or at the 
computer.""" .


###  http://www.owl-ontologies.com/VirtualHome.owl#playtime_lunch_with_dolls
ho:playtime_lunch_with_dolls rdf:type owl:Class ;
                             rdfs:subClassOf ho:Leisure ;
                             rdfs:comment """The class with sequence of actions for playing with dolls while eating 
your lunch.""" .


###  http://www.owl-ontologies.com/VirtualHome.owl#plug_in_nightlight
ho:plug_in_nightlight rdf:type owl:Class ;
                      rdfs:subClassOf ho:Other ;
                      rdfs:comment "The class with sequence of actions for pluging in the nightlight, in any room." .


###  http://www.owl-ontologies.com/VirtualHome.owl#polish_table
ho:polish_table rdf:type owl:Class ;
                rdfs:subClassOf ho:HouseCleaning ;
                rdfs:comment "The class with sequence of actions to polish a table." .


###  http://www.owl-ontologies.com/VirtualHome.owl#polish_teas_pot
ho:polish_teas_pot rdf:type owl:Class ;
                   rdfs:subClassOf ho:HouseArrangement ;
                   rdfs:comment """The class with sequence of actions for polishing tea pots
.""" .


###  http://www.owl-ontologies.com/VirtualHome.owl#polish_your_shoes
ho:polish_your_shoes rdf:type owl:Class ;
                     rdfs:subClassOf ho:HouseArrangement ;
                     rdfs:comment "The class with sequence of actions for polishing your own shoes." .


###  http://www.owl-ontologies.com/VirtualHome.owl#polishing_floor
ho:polishing_floor rdf:type owl:Class ;
                   rdfs:subClassOf ho:HouseCleaning ;
                   rdfs:comment "The class with sequence of actions for polishing the floor." .


###  http://www.owl-ontologies.com/VirtualHome.owl#pop_zit
ho:pop_zit rdf:type owl:Class ;
           rdfs:subClassOf ho:Other ;
           rdfs:comment "The class with sequence of actions for poping out zits." .


###  http://www.owl-ontologies.com/VirtualHome.owl#pour_cup_of_coffee
ho:pour_cup_of_coffee rdf:type owl:Class ;
                      rdfs:subClassOf ho:Other ;
                      rdfs:comment "The class with sequence of actions for pouring cup of coffee." .


###  http://www.owl-ontologies.com/VirtualHome.owl#practice_own_singing
ho:practice_own_singing rdf:type owl:Class ;
                        rdfs:subClassOf ho:Leisure ;
                        rdfs:comment "The class with sequence of actions for practicing your own singing." .


###  http://www.owl-ontologies.com/VirtualHome.owl#practice_violin
ho:practice_violin rdf:type owl:Class ;
                   rdfs:subClassOf ho:Leisure ;
                   rdfs:comment "The class with sequence of actions for practicing your violin." .


###  http://www.owl-ontologies.com/VirtualHome.owl#praying
ho:praying rdf:type owl:Class ;
           rdfs:subClassOf ho:Other ;
           rdfs:comment "The class with sequence of actions for praying in any room." .


###  http://www.owl-ontologies.com/VirtualHome.owl#prepare_breakfast
ho:prepare_breakfast rdf:type owl:Class ;
                     rdfs:subClassOf ho:FoodPreparation ;
                     rdfs:comment """The class with sequence of actions for preparing the breakfast (not 
eating the breakfast).""" .


###  http://www.owl-ontologies.com/VirtualHome.owl#prepare_dinner
ho:prepare_dinner rdf:type owl:Class ;
                  rdfs:subClassOf ho:FoodPreparation ;
                  rdfs:comment "Class with sequences for the procedure of getting the able ready to eat dinner." ,
                               "The class with sequence of actions for making the dinner (the procedure of cooking)." .


###  http://www.owl-ontologies.com/VirtualHome.owl#prepare_for_work
ho:prepare_for_work rdf:type owl:Class ;
                    rdfs:subClassOf ho:Work ;
                    rdfs:comment "The class with sequence of actions for preparing for work." .


###  http://www.owl-ontologies.com/VirtualHome.owl#prepare_letter_for_mailing
ho:prepare_letter_for_mailing rdf:type owl:Class ;
                              rdfs:subClassOf ho:Work ;
                              rdfs:comment """The class with sequence of actions to prepare a letter that will be send 
for mailing later.""" .


###  http://www.owl-ontologies.com/VirtualHome.owl#prepare_pot_of_boiling_water
ho:prepare_pot_of_boiling_water rdf:type owl:Class ;
                                rdfs:subClassOf ho:FoodPreparation ;
                                rdfs:comment "The class with sequence of actions for prepareing pot of boiling water." .


###  http://www.owl-ontologies.com/VirtualHome.owl#prepare_sandwich
ho:prepare_sandwich rdf:type owl:Class ;
                    rdfs:subClassOf ho:FoodPreparation ;
                    rdfs:comment "The class with sequence of actions for food preparation." .


###  http://www.owl-ontologies.com/VirtualHome.owl#prepare_sandwitch
ho:prepare_sandwitch rdf:type owl:Class ;
                     rdfs:subClassOf ho:FoodPreparation ;
                     rdfs:comment "The class with sequence of actions for preparing a sandwich." .


###  http://www.owl-ontologies.com/VirtualHome.owl#pretend_tea
ho:pretend_tea rdf:type owl:Class ;
               rdfs:subClassOf ho:Other ;
               rdfs:comment "The class with sequence of actions for pretending that you are drinking tea." .


###  http://www.owl-ontologies.com/VirtualHome.owl#print_documents
ho:print_documents rdf:type owl:Class ;
                   rdfs:subClassOf ho:Work ;
                   rdfs:comment "The class with sequence of actions for printing more than one documents." .


###  http://www.owl-ontologies.com/VirtualHome.owl#print_out_document
ho:print_out_document rdf:type owl:Class ;
                      rdfs:subClassOf ho:Work ;
                      rdfs:comment """The class with sequence of actions to print out a document, no matter 
what document.""" .


###  http://www.owl-ontologies.com/VirtualHome.owl#print_out_papers
ho:print_out_papers rdf:type owl:Class ;
                    rdfs:subClassOf ho:Work ;
                    rdfs:comment """The class with sequence of actions for printing out papers, no matter 
what type of paper.""" .


###  http://www.owl-ontologies.com/VirtualHome.owl#pull_hair_out_of_drain
ho:pull_hair_out_of_drain rdf:type owl:Class ;
                          rdfs:subClassOf ho:HouseCleaning ;
                          rdfs:comment "The class with sequence of actions for pulling the hair out of drain." .


###  http://www.owl-ontologies.com/VirtualHome.owl#pull_up_carpet
ho:pull_up_carpet rdf:type owl:Class ;
                  rdfs:subClassOf ho:Other ;
                  rdfs:comment "The class with sequence of actions for pulling up th carpet, form any room." .


###  http://www.owl-ontologies.com/VirtualHome.owl#push_all_chairs_in
ho:push_all_chairs_in rdf:type owl:Class ;
                      rdfs:subClassOf ho:HouseArrangement ;
                      rdfs:comment "The class with sequence of actions for pushing all chairs in (under the table, or other place)." .


###  http://www.owl-ontologies.com/VirtualHome.owl#push_in_desk_chair
ho:push_in_desk_chair rdf:type owl:Class ;
                      rdfs:subClassOf ho:Other ;
                      rdfs:comment "The class with sequence of actions for pushing in the desk chair." .


###  http://www.owl-ontologies.com/VirtualHome.owl#push_in_dining_room_chair
ho:push_in_dining_room_chair rdf:type owl:Class ;
                             rdfs:subClassOf ho:Other ;
                             rdfs:comment """The class with sequence of actions for pushing in the dining room chair, 
under the table or in other place.""" .


###  http://www.owl-ontologies.com/VirtualHome.owl#put_alarm_clock_in_bedroom
ho:put_alarm_clock_in_bedroom rdf:type owl:Class ;
                              rdfs:subClassOf ho:BedTimeSleep ;
                              rdfs:comment """The class with sequence of actions for setting the alarm clock at 
specific time, which exists in the bedroom.""" .


###  http://www.owl-ontologies.com/VirtualHome.owl#put_away_blankets
ho:put_away_blankets rdf:type owl:Class ;
                     rdfs:subClassOf ho:Other ;
                     rdfs:comment "The class with sequence of actions for putting away blankets." .


###  http://www.owl-ontologies.com/VirtualHome.owl#put_away_clean_clothes
ho:put_away_clean_clothes rdf:type owl:Class ;
                          rdfs:subClassOf ho:HouseArrangement ;
                          rdfs:comment "The class with sequence of actions for for putting away clean clothes." .


###  http://www.owl-ontologies.com/VirtualHome.owl#put_away_clothes
ho:put_away_clothes rdf:type owl:Class ;
                    rdfs:subClassOf ho:Other ;
                    rdfs:comment "The class with sequence of actions for putting away clothes." .


###  http://www.owl-ontologies.com/VirtualHome.owl#put_away_dishes
ho:put_away_dishes rdf:type owl:Class ;
                   rdfs:subClassOf ho:HouseArrangement ;
                   rdfs:comment "The class with sequence of actions for putting away the dishes." .


###  http://www.owl-ontologies.com/VirtualHome.owl#put_away_groceries
ho:put_away_groceries rdf:type owl:Class ;
                      rdfs:subClassOf ho:HouseArrangement ;
                      rdfs:comment """The class with sequence of actions for putting away the groceries, not 
in specific room.""" .


###  http://www.owl-ontologies.com/VirtualHome.owl#put_away_jackets
ho:put_away_jackets rdf:type owl:Class ;
                    rdfs:subClassOf ho:Other ;
                    rdfs:comment "The class with sequence of actions for putting away the jackets." .


###  http://www.owl-ontologies.com/VirtualHome.owl#put_away_keys
ho:put_away_keys rdf:type owl:Class ;
                 rdfs:subClassOf ho:Other ;
                 rdfs:comment """The class with sequence of actions for putting away keys, in their 
storing place.""" .


###  http://www.owl-ontologies.com/VirtualHome.owl#put_away_shoes
ho:put_away_shoes rdf:type owl:Class ;
                  rdfs:subClassOf ho:Other ;
                  rdfs:comment "The class with sequence of actions for putting away the shoes." .


###  http://www.owl-ontologies.com/VirtualHome.owl#put_away_toys
ho:put_away_toys rdf:type owl:Class ;
                 rdfs:subClassOf ho:Other ;
                 rdfs:comment "The class with sequence of actions for putting away the toys." .


###  http://www.owl-ontologies.com/VirtualHome.owl#put_clothes_away
ho:put_clothes_away rdf:type owl:Class ;
                    rdfs:subClassOf ho:Other ;
                    rdfs:comment "The class with sequence of actions for putting clothes away." .


###  http://www.owl-ontologies.com/VirtualHome.owl#put_dishes_away
ho:put_dishes_away rdf:type owl:Class ;
                   rdfs:subClassOf ho:HouseArrangement ;
                   rdfs:comment """The class with sequence of actions for putting dishes away from any 
place.""" .


###  http://www.owl-ontologies.com/VirtualHome.owl#put_down_bags
ho:put_down_bags rdf:type owl:Class ;
                 rdfs:subClassOf ho:Other ;
                 rdfs:comment "The class with sequence of actions for putting down bags, in any room." .


###  http://www.owl-ontologies.com/VirtualHome.owl#put_down_decoration
ho:put_down_decoration rdf:type owl:Class ;
                       rdfs:subClassOf ho:HouseArrangement ;
                       rdfs:comment """The class with sequence of actions for putting down decoration, on the 
floor or table.""" .


###  http://www.owl-ontologies.com/VirtualHome.owl#put_dvds_on_shelves
ho:put_dvds_on_shelves rdf:type owl:Class ;
                       rdfs:subClassOf ho:HouseArrangement ;
                       rdfs:comment """The class with sequence of actions for putting the dvds on shelves
.""" .


###  http://www.owl-ontologies.com/VirtualHome.owl#put_groceries_in_fridge
ho:put_groceries_in_fridge rdf:type owl:Class ;
                           rdfs:subClassOf ho:HouseArrangement ;
                           rdfs:comment """Class with sequences that show how to put groceries and other object in 
the fridge.""" .


###  http://www.owl-ontologies.com/VirtualHome.owl#put_in_chair
ho:put_in_chair rdf:type owl:Class ;
                rdfs:subClassOf ho:Other ;
                rdfs:comment """The class with sequence of actions for putting in the chair or chairs in 
any room.""" .


###  http://www.owl-ontologies.com/VirtualHome.owl#put_mail_away
ho:put_mail_away rdf:type owl:Class ;
                 rdfs:subClassOf ho:HouseArrangement ;
                 rdfs:comment """The class with sequence of actions for putiing mails away, in a specific 
place.""" .


###  http://www.owl-ontologies.com/VirtualHome.owl#put_mail_in_mail_organizer
ho:put_mail_in_mail_organizer rdf:type owl:Class ;
                              rdfs:subClassOf ho:HouseArrangement ;
                              rdfs:comment "The class with sequence of actions for puttin mail in mail organizer." .


###  http://www.owl-ontologies.com/VirtualHome.owl#put_new_books_in_shelves
ho:put_new_books_in_shelves rdf:type owl:Class ;
                            rdfs:subClassOf ho:HouseArrangement ;
                            rdfs:comment """The class with sequence of actions for putting new books in shelves, 
from another place.""" .


###  http://www.owl-ontologies.com/VirtualHome.owl#put_on_coat
ho:put_on_coat rdf:type owl:Class ;
               rdfs:subClassOf ho:HygieneStyling ;
               rdfs:comment "The class with sequence of actions for putting on your coat." .


###  http://www.owl-ontologies.com/VirtualHome.owl#put_on_coat_and_shoes
ho:put_on_coat_and_shoes rdf:type owl:Class ;
                         rdfs:subClassOf ho:HygieneStyling ;
                         rdfs:comment "The class with sequence of actions for putiing on coat and shoes." .


###  http://www.owl-ontologies.com/VirtualHome.owl#put_on_foundation
ho:put_on_foundation rdf:type owl:Class ;
                     rdfs:subClassOf ho:HygieneStyling ;
                     rdfs:comment "The class with sequence of actions for putting on a foundation." .


###  http://www.owl-ontologies.com/VirtualHome.owl#put_on_glasses
ho:put_on_glasses rdf:type owl:Class ;
                  rdfs:subClassOf ho:HygieneStyling ;
                  rdfs:comment "The class with sequence of actions for putting your glasses on." .


###  http://www.owl-ontologies.com/VirtualHome.owl#put_on_purse_put_keys_and_lucky_charms_in_pockets_leave_home
ho:put_on_purse_put_keys_and_lucky_charms_in_pockets_leave_home rdf:type owl:Class ;
                                                                rdfs:subClassOf ho:Other ;
                                                                rdfs:comment """The class with sequence of actions for putting on purse, putting keys 
and lucjy charm in pockets, and leave home.""" .


###  http://www.owl-ontologies.com/VirtualHome.owl#put_on_your_shoes
ho:put_on_your_shoes rdf:type owl:Class ;
                     rdfs:subClassOf ho:HygieneStyling ;
                     rdfs:comment """The class with sequence of actions for putiing on your shoes, in any 
room.""" .


###  http://www.owl-ontologies.com/VirtualHome.owl#put_out_flowers
ho:put_out_flowers rdf:type owl:Class ;
                   rdfs:subClassOf ho:Other ;
                   rdfs:comment "The class with sequence of actions for putting out flowers on the balcony, or some external place of the house." .


###  http://www.owl-ontologies.com/VirtualHome.owl#put_shoes_and_coats
ho:put_shoes_and_coats rdf:type owl:Class ;
                       rdfs:subClassOf ho:HygieneStyling ;
                       rdfs:comment "The class with sequence of actions for putting shoes and coats." .


###  http://www.owl-ontologies.com/VirtualHome.owl#put_shoes_in_shoe_rack
ho:put_shoes_in_shoe_rack rdf:type owl:Class ;
                          rdfs:subClassOf ho:HouseArrangement ;
                          rdfs:comment "The class with sequence of actions for putting the shoes in shoe rack, wherever the shoe rack is." .


###  http://www.owl-ontologies.com/VirtualHome.owl#put_slippers_in_closet
ho:put_slippers_in_closet rdf:type owl:Class ;
                          rdfs:subClassOf ho:HouseArrangement ;
                          rdfs:comment """The class with sequence of actions for putting slippers in closet, in 
any room the closet is.""" .


###  http://www.owl-ontologies.com/VirtualHome.owl#put_them_to_sleep
ho:put_them_to_sleep rdf:type owl:Class ;
                     rdfs:subClassOf ho:BedTimeSleep ;
                     rdfs:comment "The class with sequence of actions for putting them to sleep." .


###  http://www.owl-ontologies.com/VirtualHome.owl#put_toys_away
ho:put_toys_away rdf:type owl:Class ;
                 rdfs:subClassOf ho:HouseArrangement ;
                 rdfs:comment """The class with sequence of actions for putting the toys away, that 
belong to childeren or your own.""" .


###  http://www.owl-ontologies.com/VirtualHome.owl#put_umbrella_away
ho:put_umbrella_away rdf:type owl:Class ;
                     rdfs:subClassOf ho:Other ;
                     rdfs:comment """The class with sequence of actions for putting the umbrella away, in any 
place.""" .


###  http://www.owl-ontologies.com/VirtualHome.owl#put_up_coat
ho:put_up_coat rdf:type owl:Class ;
               rdfs:subClassOf ho:HygieneStyling ;
               rdfs:comment """<p style=\"margin-top: 0\">
      The class with sequence of actions for putting up coat.
    </p>""" .


###  http://www.owl-ontologies.com/VirtualHome.owl#put_up_decoration
ho:put_up_decoration rdf:type owl:Class ;
                     rdfs:subClassOf ho:Other ;
                     rdfs:comment "The class with sequence of actions for putting up decoration." .


###  http://www.owl-ontologies.com/VirtualHome.owl#put_up_feet
ho:put_up_feet rdf:type owl:Class ;
               rdfs:subClassOf ho:Other ;
               rdfs:comment "The class with sequence of actions for putting up your feet, in any place and room." .


###  http://www.owl-ontologies.com/VirtualHome.owl#put_up_jacket
ho:put_up_jacket rdf:type owl:Class ;
                 rdfs:subClassOf ho:Other ;
                 rdfs:comment "The class with sequence of actions for putting up a jacket, in any room." .


###  http://www.owl-ontologies.com/VirtualHome.owl#put_up_towel
ho:put_up_towel rdf:type owl:Class ;
                rdfs:subClassOf ho:Other ;
                rdfs:comment """The class with sequence of actions for putting up towel, in any room on 
you.""" .


###  http://www.owl-ontologies.com/VirtualHome.owl#put_washed_clothes_in_almirah
ho:put_washed_clothes_in_almirah rdf:type owl:Class ;
                                 rdfs:subClassOf ho:HouseArrangement ;
                                 rdfs:comment "The class with sequence of actions for putting washed clothes in almirah." .


###  http://www.owl-ontologies.com/VirtualHome.owl#rain_welcome
ho:rain_welcome rdf:type owl:Class ;
                rdfs:subClassOf ho:Other ;
                rdfs:comment """he class with sequence of actions for raining welcome (comming inside 
the house, after rain).""" .


###  http://www.owl-ontologies.com/VirtualHome.owl#raise_blinds
ho:raise_blinds rdf:type owl:Class ;
                rdfs:subClassOf ho:Other ;
                rdfs:comment """The class with sequence of actions for raising blinds, from any window in any room.
    </p>""" .


###  http://www.owl-ontologies.com/VirtualHome.owl#re_arrange_office
ho:re_arrange_office rdf:type owl:Class ;
                     rdfs:subClassOf ho:HouseArrangement ;
                     rdfs:comment """The class with sequence of actions for re arranging office, cleaning or 
sorting items, etc.""" .


###  http://www.owl-ontologies.com/VirtualHome.owl#read_book
ho:read_book rdf:type owl:Class ;
             rdfs:subClassOf ho:Leisure ;
             rdfs:comment "Class which contains sequence of action, about how to read of a book." .


###  http://www.owl-ontologies.com/VirtualHome.owl#read_magazine
ho:read_magazine rdf:type owl:Class ;
                 rdfs:subClassOf ho:Leisure ;
                 rdfs:comment """The class with sequence of actions for reading a magazine (not a 
newspaper).""" .


###  http://www.owl-ontologies.com/VirtualHome.owl#read_news
ho:read_news rdf:type owl:Class ;
             rdfs:subClassOf ho:Leisure ;
             rdfs:comment """The class with sequence of actions for reading news (either from a 
newspaper, either from the internet).""" .


###  http://www.owl-ontologies.com/VirtualHome.owl#read_newspaper
ho:read_newspaper rdf:type owl:Class ;
                  rdfs:subClassOf ho:Leisure ;
                  rdfs:comment "The class with sequence of actions for reading a newspaper." .


###  http://www.owl-ontologies.com/VirtualHome.owl#read_on_sofa
ho:read_on_sofa rdf:type owl:Class ;
                rdfs:subClassOf ho:Leisure ;
                rdfs:comment """The class with sequence of actions reading womehting (newspaper, or 
book or magazine), while on the sofa.""" .


###  http://www.owl-ontologies.com/VirtualHome.owl#read_paper
ho:read_paper rdf:type owl:Class ;
              rdfs:subClassOf ho:Work ;
              rdfs:comment "The class with sequence of actions for reading some kind of paper." .


###  http://www.owl-ontologies.com/VirtualHome.owl#read_text_message
ho:read_text_message rdf:type owl:Class ;
                     rdfs:subClassOf ho:Other ;
                     rdfs:comment """The class with sequence of actions for reading text message, form the 
phone, or computer.""" .


###  http://www.owl-ontologies.com/VirtualHome.owl#read_them_bedtime_story
ho:read_them_bedtime_story rdf:type owl:Class ;
                           rdfs:subClassOf ho:BedTimeSleep ;
                           rdfs:comment """The class with sequence of actions for reading to someone lese a bedtime 
story.""" .


###  http://www.owl-ontologies.com/VirtualHome.owl#read_to_child
ho:read_to_child rdf:type owl:Class ;
                 rdfs:subClassOf ho:SocialInteraction ;
                 rdfs:comment "The class with sequence of actions for readin to your child in any room." .


###  http://www.owl-ontologies.com/VirtualHome.owl#read_yourself_to_sleep
ho:read_yourself_to_sleep rdf:type owl:Class ;
                          rdfs:subClassOf ho:Leisure ;
                          rdfs:comment """The class with sequence of actions for reading and falling to sleep 
while reading.""" .


###  http://www.owl-ontologies.com/VirtualHome.owl#rearrange_photo_frames
ho:rearrange_photo_frames rdf:type owl:Class ;
                          rdfs:subClassOf ho:HouseArrangement ;
                          rdfs:comment "The class with sequence of actions for rearranging photo frames." .


###  http://www.owl-ontologies.com/VirtualHome.owl#receive_credit_card
ho:receive_credit_card rdf:type owl:Class ;
                       rdfs:subClassOf ho:Other ;
                       rdfs:comment "The class with sequence of actions for receiving a credit card." .


###  http://www.owl-ontologies.com/VirtualHome.owl#recycle_items
ho:recycle_items rdf:type owl:Class ;
                 rdfs:subClassOf ho:Other ;
                 rdfs:comment "The class with sequence of actions for recycling items." .


###  http://www.owl-ontologies.com/VirtualHome.owl#relax
ho:relax rdf:type owl:Class ;
         rdfs:subClassOf ho:Leisure ;
         rdfs:comment "The class with sequence of actions for relaxing." .


###  http://www.owl-ontologies.com/VirtualHome.owl#relax_on_sofa
ho:relax_on_sofa rdf:type owl:Class ;
                 rdfs:subClassOf ho:Leisure ;
                 rdfs:comment "This class contains sequence of actions on how you can relax on a sofa." .


###  http://www.owl-ontologies.com/VirtualHome.owl#replace_toothpaste
ho:replace_toothpaste rdf:type owl:Class ;
                      rdfs:subClassOf ho:HouseArrangement ;
                      rdfs:comment """The class with sequence of actions for replacing the toohtpaste in any 
room.""" .


###  http://www.owl-ontologies.com/VirtualHome.owl#replace_towel
ho:replace_towel rdf:type owl:Class ;
                 rdfs:subClassOf ho:Other ;
                 rdfs:comment "The class with sequence of actions for replacing a towel, from any room." .


###  http://www.owl-ontologies.com/VirtualHome.owl#research
ho:research rdf:type owl:Class ;
            rdfs:subClassOf ho:Work ;
            rdfs:comment "The class with sequence of actions for performing research." .


###  http://www.owl-ontologies.com/VirtualHome.owl#restock
ho:restock rdf:type owl:Class ;
           rdfs:subClassOf ho:Other ;
           rdfs:comment "The class with sequence of actions for restocking, any place." .


###  http://www.owl-ontologies.com/VirtualHome.owl#return_from_store
ho:return_from_store rdf:type owl:Class ;
                     rdfs:subClassOf ho:Other ;
                     rdfs:comment "The class with sequence of actions for returning from the store." .


###  http://www.owl-ontologies.com/VirtualHome.owl#return_phone_calls
ho:return_phone_calls rdf:type owl:Class ;
                      rdfs:subClassOf ho:Other ;
                      rdfs:comment """The class with sequence of actions for returning phone calls, either 
from your cell phone or home phone.""" .


###  http://www.owl-ontologies.com/VirtualHome.owl#rotate_stock_in_refrigerator
ho:rotate_stock_in_refrigerator rdf:type owl:Class ;
                                rdfs:subClassOf ho:HouseArrangement ;
                                rdfs:comment "The class with sequence of actions for rotating stock in Refrigerator." .


###  http://www.owl-ontologies.com/VirtualHome.owl#say_goodbye
ho:say_goodbye rdf:type owl:Class ;
               rdfs:subClassOf ho:SocialInteraction ;
               rdfs:comment "The class with sequence of actions for greeding by saying goodbye." .


###  http://www.owl-ontologies.com/VirtualHome.owl#say_goodbye_to_guests_leaving
ho:say_goodbye_to_guests_leaving rdf:type owl:Class ;
                                 rdfs:subClassOf ho:SocialInteraction ;
                                 rdfs:comment "The class with sequence of actions for saying goodbye to guests leaving." .


###  http://www.owl-ontologies.com/VirtualHome.owl#scrub_bottom_of_feet
ho:scrub_bottom_of_feet rdf:type owl:Class ;
                        rdfs:subClassOf ho:HygieneStyling ;
                        rdfs:comment "The class with sequence of actions for scrubbing just the bottom of your feet." .


###  http://www.owl-ontologies.com/VirtualHome.owl#scrub_face
ho:scrub_face rdf:type owl:Class ;
              rdfs:subClassOf ho:HygieneStyling ;
              rdfs:comment "The class with sequence of actions for scrubing you face." .


###  http://www.owl-ontologies.com/VirtualHome.owl#scrub_toilet
ho:scrub_toilet rdf:type owl:Class ;
                rdfs:subClassOf ho:HouseCleaning ;
                rdfs:comment "The class with sequence of actions for scrubing the toilet." .


###  http://www.owl-ontologies.com/VirtualHome.owl#scrubbing_living_room_tile_floor_is_once_week_activity_for_me
ho:scrubbing_living_room_tile_floor_is_once_week_activity_for_me rdf:type owl:Class ;
                                                                 rdfs:subClassOf ho:HouseCleaning ;
                                                                 rdfs:comment "The class with sequence of actions for scrubbing living room tile floor is once a week activity for me." .


###  http://www.owl-ontologies.com/VirtualHome.owl#send__email
ho:send__email rdf:type owl:Class ;
               rdfs:subClassOf ho:Work ;
               rdfs:comment "The class with sequence of actions for sending an email." .


###  http://www.owl-ontologies.com/VirtualHome.owl#sent_email
ho:sent_email rdf:type owl:Class ;
              rdfs:subClassOf ho:Work ;
              rdfs:comment "The class with sequence of actions to send a email." .


###  http://www.owl-ontologies.com/VirtualHome.owl#serve_breakfast
ho:serve_breakfast rdf:type owl:Class ;
                   rdfs:subClassOf ho:Other ;
                   rdfs:comment "The class with sequence of actions for serving breakfast, in any room." .


###  http://www.owl-ontologies.com/VirtualHome.owl#serve_cookies
ho:serve_cookies rdf:type owl:Class ;
                 rdfs:subClassOf ho:Other ;
                 rdfs:comment "The class with sequence of actions for serving cookies, for any occasion." .


###  http://www.owl-ontologies.com/VirtualHome.owl#serve_food
ho:serve_food rdf:type owl:Class ;
              rdfs:subClassOf ho:Other ;
              rdfs:comment "The class with sequence of actions for serving the food in any room." .


###  http://www.owl-ontologies.com/VirtualHome.owl#serve_hors_doeurves_to_entering_guests_at_cocktail_party
ho:serve_hors_doeurves_to_entering_guests_at_cocktail_party rdf:type owl:Class ;
                                                            rdfs:subClassOf ho:SocialInteraction ;
                                                            rdfs:comment "The class with sequence of actions for srving hors doeurves to entering guest at cocktail party." .


###  http://www.owl-ontologies.com/VirtualHome.owl#serve_meal
ho:serve_meal rdf:type owl:Class ;
              rdfs:subClassOf ho:Other ;
              rdfs:comment "The class with sequence of actions for serving meal in any room." .


###  http://www.owl-ontologies.com/VirtualHome.owl#set_mail_on_table
ho:set_mail_on_table rdf:type owl:Class ;
                     rdfs:subClassOf ho:Other ;
                     rdfs:comment "The class with sequence of actions for setting the mail on the table, for eating." .


###  http://www.owl-ontologies.com/VirtualHome.owl#set_out_some_snacks_for_toddler
ho:set_out_some_snacks_for_toddler rdf:type owl:Class ;
                                   rdfs:subClassOf ho:Other ;
                                   rdfs:comment "The class with sequence of actions for setting out some snacks for toddler." .


###  http://www.owl-ontologies.com/VirtualHome.owl#set_up_buffet_area
ho:set_up_buffet_area rdf:type owl:Class ;
                      rdfs:subClassOf ho:HouseArrangement ;
                      rdfs:comment "The class with sequence of actions for setting up the buffet area." .


###  http://www.owl-ontologies.com/VirtualHome.owl#set_up_table
ho:set_up_table rdf:type owl:Class ;
                rdfs:subClassOf ho:HouseArrangement ;
                rdfs:comment "Class with sequences about how to perform the set up of a dinner, kitchen table." .


###  http://www.owl-ontologies.com/VirtualHome.owl#set_up_tv
ho:set_up_tv rdf:type owl:Class ;
             rdfs:subClassOf ho:Other ;
             rdfs:comment "The class with sequence of actions for seeting up the TV." .


###  http://www.owl-ontologies.com/VirtualHome.owl#settle_in
ho:settle_in rdf:type owl:Class ;
             rdfs:subClassOf ho:Other ;
             rdfs:comment "The class with sequence of actions for settling in the house." .


###  http://www.owl-ontologies.com/VirtualHome.owl#sew_button
ho:sew_button rdf:type owl:Class ;
              rdfs:subClassOf ho:Other ;
              rdfs:comment """The class with sequence of actions for sewing the button, from any 
remote control.""" .


###  http://www.owl-ontologies.com/VirtualHome.owl#shampoo_hair
ho:shampoo_hair rdf:type owl:Class ;
                rdfs:subClassOf ho:HygieneStyling ;
                rdfs:comment "The class with sequence of actions for shampooing your hair." .


###  http://www.owl-ontologies.com/VirtualHome.owl#shoe_removal
ho:shoe_removal rdf:type owl:Class ;
                rdfs:subClassOf ho:Other ;
                rdfs:comment "The class with sequence of actions for removing your shoes in any room." .


###  http://www.owl-ontologies.com/VirtualHome.owl#shop
ho:shop rdf:type owl:Class ;
        rdfs:subClassOf ho:Other ;
        rdfs:comment """The class with sequence of actions for shopping either by calling, or 
from the internet (shopping from household environment).""" .


###  http://www.owl-ontologies.com/VirtualHome.owl#shred_receipts
ho:shred_receipts rdf:type owl:Class ;
                  rdfs:subClassOf ho:HouseCleaning ;
                  rdfs:comment "The class with sequence of actions for shred of receipts." .


###  http://www.owl-ontologies.com/VirtualHome.owl#shredding
ho:shredding rdf:type owl:Class ;
             rdfs:subClassOf ho:Other ;
             rdfs:comment "The class with sequence of actions for shredding any object in any room." .


###  http://www.owl-ontologies.com/VirtualHome.owl#shut_front_door
ho:shut_front_door rdf:type owl:Class ;
                   rdfs:subClassOf ho:Other ;
                   rdfs:comment "The class with sequence of actions for shutting front door (door of main entrance)." .


###  http://www.owl-ontologies.com/VirtualHome.owl#shut_off_alarm
ho:shut_off_alarm rdf:type owl:Class ;
                  rdfs:subClassOf ho:Other ;
                  rdfs:comment "The class with sequence of actions for shutting of the alarm in any room." .


###  http://www.owl-ontologies.com/VirtualHome.owl#sing_karaoke
ho:sing_karaoke rdf:type owl:Class ;
                rdfs:subClassOf ho:Leisure ;
                rdfs:comment "The class with sequence of actions for singing at the karoke." .


###  http://www.owl-ontologies.com/VirtualHome.owl#sing_song
ho:sing_song rdf:type owl:Class ;
             rdfs:subClassOf ho:Leisure ;
             rdfs:comment "The class with sequence of actions for singing songs." .


###  http://www.owl-ontologies.com/VirtualHome.owl#sit_in_chair
ho:sit_in_chair rdf:type owl:Class ;
                rdfs:subClassOf ho:Other ;
                rdfs:comment """The class with sequence of actions for sitting in the chair, in any type 
of chair in any room.""" .


###  http://www.owl-ontologies.com/VirtualHome.owl#sit_quietly
ho:sit_quietly rdf:type owl:Class ;
               rdfs:subClassOf ho:Other ;
               rdfs:comment "The class with sequence of actions for sitting quetly, in any room." .


###  http://www.owl-ontologies.com/VirtualHome.owl#sleep
ho:sleep rdf:type owl:Class ;
         rdfs:subClassOf ho:BedTimeSleep ;
         rdfs:comment "The class with sequence of actions for sleeping." .


###  http://www.owl-ontologies.com/VirtualHome.owl#slice_apple
ho:slice_apple rdf:type owl:Class ;
               rdfs:subClassOf ho:FoodPreparation ;
               rdfs:comment "The class with sequence of actions for slicing an apple." .


###  http://www.owl-ontologies.com/VirtualHome.owl#social_media__checks
ho:social_media__checks rdf:type owl:Class ;
                        rdfs:subClassOf ho:Leisure ;
                        rdfs:comment """The class with sequence of actions for chencking your social media 
applications.""" .


###  http://www.owl-ontologies.com/VirtualHome.owl#sort_and_fold_laundry
ho:sort_and_fold_laundry rdf:type owl:Class ;
                         rdfs:subClassOf ho:HouseCleaning ;
                         rdfs:comment "The class with sequence of actions for sorting and folding laundry." .


###  http://www.owl-ontologies.com/VirtualHome.owl#sort_clothing_and_care_for_it
ho:sort_clothing_and_care_for_it rdf:type owl:Class ;
                                 rdfs:subClassOf ho:HouseArrangement ;
                                 rdfs:comment "The class with sequence of actions for sorting clothing in specific order." .


###  http://www.owl-ontologies.com/VirtualHome.owl#sort_laundry
ho:sort_laundry rdf:type owl:Class ;
                rdfs:subClassOf ho:HouseArrangement ;
                rdfs:comment "The class with sequence of actions for sorting laundry by category." .


###  http://www.owl-ontologies.com/VirtualHome.owl#sort_mail
ho:sort_mail rdf:type owl:Class ;
             rdfs:subClassOf ho:Other ;
             rdfs:comment """The class with sequence of actions for sorting mail, in any desired 
order.""" .


###  http://www.owl-ontologies.com/VirtualHome.owl#speaking_on_headset_in_skype_or_some_form_of_voip_for_business_call
ho:speaking_on_headset_in_skype_or_some_form_of_voip_for_business_call rdf:type owl:Class ;
                                                                       rdfs:subClassOf ho:SocialInteraction ,
                                                                                       ho:Work ;
                                                                       rdfs:comment """The class with sequence of actions for speaking on headset in skype or 
some form of voip for business call.""" ,
                                                                                    "The class with sequence of actions for speaking on headset in skype or some form of voip for business call." .


###  http://www.owl-ontologies.com/VirtualHome.owl#spend_family_time_playing_games
ho:spend_family_time_playing_games rdf:type owl:Class ;
                                   rdfs:subClassOf ho:SocialInteraction ;
                                   rdfs:comment "The class with sequence of actions for spending family time playing games, videogames of any other games." .


###  http://www.owl-ontologies.com/VirtualHome.owl#spread_table_with_appropriate_supplies
ho:spread_table_with_appropriate_supplies rdf:type owl:Class ;
                                          rdfs:subClassOf ho:Other ;
                                          rdfs:comment """The class with sequence of actions for spreading the table with 
approproate supplies.""" .


###  http://www.owl-ontologies.com/VirtualHome.owl#squeeze_lemon
ho:squeeze_lemon rdf:type owl:Class ;
                 rdfs:subClassOf ho:FoodPreparation ;
                 rdfs:comment "The class with sequence of actions for squezing a lemon." .


###  http://www.owl-ontologies.com/VirtualHome.owl#start_computer
ho:start_computer rdf:type owl:Class ;
                  rdfs:subClassOf ho:Other ;
                  rdfs:comment """The class with sequence of actions for starting your computer, either 
laptop or personal computer.""" .


###  http://www.owl-ontologies.com/VirtualHome.owl#steam_mop_floor
ho:steam_mop_floor rdf:type owl:Class ;
                   rdfs:subClassOf ho:HouseCleaning ;
                   rdfs:comment "The class with sequence of actions for steaming mop floor." .


###  http://www.owl-ontologies.com/VirtualHome.owl#story_reading_time
ho:story_reading_time rdf:type owl:Class ;
                      rdfs:subClassOf ho:SocialInteraction ;
                      rdfs:comment "The class with sequence of actions for story reading time, in any room." .


###  http://www.owl-ontologies.com/VirtualHome.owl#straighten_bookshelf
ho:straighten_bookshelf rdf:type owl:Class ;
                        rdfs:subClassOf ho:Other ;
                        rdfs:comment """The class with sequence of actions for straightening the bookself, in 
any room.""" .


###  http://www.owl-ontologies.com/VirtualHome.owl#straighten_magazines
ho:straighten_magazines rdf:type owl:Class ;
                        rdfs:subClassOf ho:HouseArrangement ;
                        rdfs:comment """The class with sequence of actions for straighten magaziens that are 
placed in a folder or on a surface.""" .


###  http://www.owl-ontologies.com/VirtualHome.owl#straighten_paintings_on_wall
ho:straighten_paintings_on_wall rdf:type owl:Class ;
                                rdfs:subClassOf ho:HouseArrangement ;
                                rdfs:comment """The class with sequence of actions for straightening paintings on wall 
(only painting not pictures).""" .


###  http://www.owl-ontologies.com/VirtualHome.owl#straighten_pictures_on_wall
ho:straighten_pictures_on_wall rdf:type owl:Class ;
                               rdfs:subClassOf ho:HouseArrangement ;
                               rdfs:comment "The class with sequence of actions for straighten pictures on wall, in any room." .


###  http://www.owl-ontologies.com/VirtualHome.owl#string_green_beans
ho:string_green_beans rdf:type owl:Class ;
                      rdfs:subClassOf ho:Other ;
                      rdfs:comment """The class with sequence of actions for stringing green beans, in any 
room.""" .


###  http://www.owl-ontologies.com/VirtualHome.owl#study
ho:study rdf:type owl:Class ;
         rdfs:subClassOf ho:Work ;
         rdfs:comment "The class with sequence of actions for studying, no matter on what (computer, paper)." .


###  http://www.owl-ontologies.com/VirtualHome.owl#study_bible
ho:study_bible rdf:type owl:Class ;
               rdfs:subClassOf ho:Work ;
               rdfs:comment "The class with sequence of actions for studying the biblie." .


###  http://www.owl-ontologies.com/VirtualHome.owl#style_hair
ho:style_hair rdf:type owl:Class ;
              rdfs:subClassOf ho:HygieneStyling ;
              rdfs:comment "The class with sequence of actions for styling your hair." .


###  http://www.owl-ontologies.com/VirtualHome.owl#surf_internet
ho:surf_internet rdf:type owl:Class ;
                 rdfs:subClassOf ho:Leisure ;
                 rdfs:comment "The class with sequence of actions for surfing the internet." .


###  http://www.owl-ontologies.com/VirtualHome.owl#surf_net
ho:surf_net rdf:type owl:Class ;
            rdfs:subClassOf ho:Leisure ;
            rdfs:comment "The class with sequence of actions for surfing the net." .


###  http://www.owl-ontologies.com/VirtualHome.owl#surf_web_for_money_legitimate_making_opportunities
ho:surf_web_for_money_legitimate_making_opportunities rdf:type owl:Class ;
                                                      rdfs:subClassOf ho:Work ;
                                                      rdfs:comment """The class with sequence of actions for searching in the internet for 
legitimate maikng opportunities.""" .


###  http://www.owl-ontologies.com/VirtualHome.owl#sweep_and_wipe_table_off_with_rag
ho:sweep_and_wipe_table_off_with_rag rdf:type owl:Class ;
                                     rdfs:subClassOf ho:HouseCleaning ;
                                     rdfs:comment """The class with sequence of actions for sweeping and wiping a table off 
with a rag.""" .


###  http://www.owl-ontologies.com/VirtualHome.owl#sweep_entrance_hall
ho:sweep_entrance_hall rdf:type owl:Class ;
                       rdfs:subClassOf ho:HouseCleaning ;
                       rdfs:comment "The class with sequence of actions on how to sweep the entrance hall." .


###  http://www.owl-ontologies.com/VirtualHome.owl#sweep_floor
ho:sweep_floor rdf:type owl:Class ;
               rdfs:subClassOf ho:HouseCleaning ;
               rdfs:comment "The class with sequence of actions for house cleaning." .


###  http://www.owl-ontologies.com/VirtualHome.owl#sweep_hallway_please
ho:sweep_hallway_please rdf:type owl:Class ;
                        rdfs:subClassOf ho:HouseCleaning ;
                        rdfs:comment """he class with sequence of actions to sweep the hallway after you got 
the verbal token \"please\".""" .


###  http://www.owl-ontologies.com/VirtualHome.owl#switch_on_lamp
ho:switch_on_lamp rdf:type owl:Class ;
                  rdfs:subClassOf ho:Other ;
                  rdfs:comment "The class with sequence of actions for switching on lamp, in any room." .


###  http://www.owl-ontologies.com/VirtualHome.owl#tabletop_game
ho:tabletop_game rdf:type owl:Class ;
                 rdfs:subClassOf ho:Leisure ;
                 rdfs:comment """The class with sequence of actions for playin tabletop games (board 
games).""" .


###  http://www.owl-ontologies.com/VirtualHome.owl#take_bath
ho:take_bath rdf:type owl:Class ;
             rdfs:subClassOf ho:HygieneStyling ;
             rdfs:comment "Class with seqeunces on how you can take a bath, and clean yourself (not a shower)." .


###  http://www.owl-ontologies.com/VirtualHome.owl#take_coat
ho:take_coat rdf:type owl:Class ;
             rdfs:subClassOf ho:Other ;
             rdfs:comment """The class with sequence of actions for taking the coat, and place it 
somewhere.""" .


###  http://www.owl-ontologies.com/VirtualHome.owl#take_dishes_out_of_dishwasher
ho:take_dishes_out_of_dishwasher rdf:type owl:Class ;
                                 rdfs:subClassOf ho:HouseArrangement ;
                                 rdfs:comment "The class with sequence of actions for taking dishes out of dishwasher." .


###  http://www.owl-ontologies.com/VirtualHome.owl#take_jacket_off
ho:take_jacket_off rdf:type owl:Class ;
                   rdfs:subClassOf ho:HygieneStyling ;
                   rdfs:comment "The class with sequence of actions for taking your jacket off." .


###  http://www.owl-ontologies.com/VirtualHome.owl#take_nap
ho:take_nap rdf:type owl:Class ;
            rdfs:subClassOf ho:BedTimeSleep ;
            rdfs:comment "A class with sequences on how to go take a small nap." .


###  http://www.owl-ontologies.com/VirtualHome.owl#take_of_outerwear
ho:take_of_outerwear rdf:type owl:Class ;
                     rdfs:subClassOf ho:Other ;
                     rdfs:comment "The class with sequence of actions for taking of outerwear." .


###  http://www.owl-ontologies.com/VirtualHome.owl#take_off_coat
ho:take_off_coat rdf:type owl:Class ;
                 rdfs:subClassOf ho:HygieneStyling ;
                 rdfs:comment "The class with sequence of actions for taking of your coat." .


###  http://www.owl-ontologies.com/VirtualHome.owl#take_off_outerwear
ho:take_off_outerwear rdf:type owl:Class ;
                      rdfs:subClassOf ho:GettingReady ;
                      rdfs:comment "The class with sequence of actions for getting ready." .


###  http://www.owl-ontologies.com/VirtualHome.owl#take_off_shoes
ho:take_off_shoes rdf:type owl:Class ;
                  rdfs:subClassOf ho:HygieneStyling ;
                  rdfs:comment """Class with seqeunces on how to take off your shoes after work, or before 
getting to bed, or watch tv.""" .


###  http://www.owl-ontologies.com/VirtualHome.owl#take_off_shoes_and_hang_up_coat
ho:take_off_shoes_and_hang_up_coat rdf:type owl:Class ;
                                   rdfs:subClassOf ho:HygieneStyling ;
                                   rdfs:comment "The class with sequence of actions for hanging up your coat." .


###  http://www.owl-ontologies.com/VirtualHome.owl#take_shoes_off
ho:take_shoes_off rdf:type owl:Class ;
                  rdfs:subClassOf ho:HygieneStyling ;
                  rdfs:comment "The class with sequence of actions for taking yur shoes off." .


###  http://www.owl-ontologies.com/VirtualHome.owl#take_shower
ho:take_shower rdf:type owl:Class ;
               rdfs:subClassOf ho:HygieneStyling ;
               rdfs:comment """Class with seqeunces of action on how to take a shower (not a bath)
.""" .


###  http://www.owl-ontologies.com/VirtualHome.owl#tale_off_shoes
ho:tale_off_shoes rdf:type owl:Class ;
                  rdfs:subClassOf ho:HygieneStyling ;
                  rdfs:comment "The class with sequence of actions for taling of your own shoes." .


###  http://www.owl-ontologies.com/VirtualHome.owl#talk_on_phone
ho:talk_on_phone rdf:type owl:Class ;
                 rdfs:subClassOf ho:SocialInteraction ;
                 rdfs:comment """The class with sequence of actions for talking on phone, either cell 
phone or phone at home.""" .


###  http://www.owl-ontologies.com/VirtualHome.owl#talk_to_kids
ho:talk_to_kids rdf:type owl:Class ;
                rdfs:subClassOf ho:SocialInteraction ;
                rdfs:comment "The class with sequence of actions for talking to kids in any room." .


###  http://www.owl-ontologies.com/VirtualHome.owl#talk_with_friends
ho:talk_with_friends rdf:type owl:Class ;
                     rdfs:subClassOf ho:SocialInteraction ;
                     rdfs:comment """The class with sequence of actions for talking to your friend, no matter 
the genre.""" .


###  http://www.owl-ontologies.com/VirtualHome.owl#talk_with_guest
ho:talk_with_guest rdf:type owl:Class ;
                   rdfs:subClassOf ho:SocialInteraction ;
                   rdfs:comment "The class with sequence of actions for talking to guest." .


###  http://www.owl-ontologies.com/VirtualHome.owl#talk_with_your_child_about_their_day
ho:talk_with_your_child_about_their_day rdf:type owl:Class ;
                                        rdfs:subClassOf ho:SocialInteraction ;
                                        rdfs:comment """The class with sequence of actions for talking with your child about 
their day.""" .


###  http://www.owl-ontologies.com/VirtualHome.owl#tax_filing
ho:tax_filing rdf:type owl:Class ;
              rdfs:subClassOf ho:Work ;
              rdfs:comment "The class with sequence of actions for filling your taxes." .


###  http://www.owl-ontologies.com/VirtualHome.owl#teach_them_to_make_their_bed
ho:teach_them_to_make_their_bed rdf:type owl:Class ;
                                rdfs:subClassOf ho:Other ;
                                rdfs:comment """The class with sequence of actions for teaching them (other persons), to 
make their beds.""" .


###  http://www.owl-ontologies.com/VirtualHome.owl#tell_jokes
ho:tell_jokes rdf:type owl:Class ;
              rdfs:subClassOf ho:SocialInteraction ;
              rdfs:comment "The class with sequence of actions for telling jokes to any individual." .


###  http://www.owl-ontologies.com/VirtualHome.owl#text_friend
ho:text_friend rdf:type owl:Class ;
               rdfs:subClassOf ho:SocialInteraction ;
               rdfs:comment "The class with sequence of actions for texting a friend." .


###  http://www.owl-ontologies.com/VirtualHome.owl#text_friends_while_sitting_on_couch
ho:text_friends_while_sitting_on_couch rdf:type owl:Class ;
                                       rdfs:subClassOf ho:SocialInteraction ;
                                       rdfs:comment """The class with sequence of actions for texting a frined while you are 
sitting on the couch.""" .


###  http://www.owl-ontologies.com/VirtualHome.owl#thanksgiving
ho:thanksgiving rdf:type owl:Class ;
                rdfs:subClassOf ho:SocialInteraction ;
                rdfs:comment "The class with sequence of actions for thanksgiving." .


###  http://www.owl-ontologies.com/VirtualHome.owl#throw_away_newspaper
ho:throw_away_newspaper rdf:type owl:Class ;
                        rdfs:subClassOf ho:Other ;
                        rdfs:comment """The class with sequence of actions for throwing away newspaper, in the 
garbage can, or elsewhere.""" .


###  http://www.owl-ontologies.com/VirtualHome.owl#throw_away_paper
ho:throw_away_paper rdf:type owl:Class ;
                    rdfs:subClassOf ho:Other ;
                    rdfs:comment """The class with sequence of actions for throwing away paper, in the 
garbage that could be in any room.""" .


###  http://www.owl-ontologies.com/VirtualHome.owl#throw_shoes
ho:throw_shoes rdf:type owl:Class ;
               rdfs:subClassOf ho:Other ;
               rdfs:comment "The class with sequence of actions for throwing away shoes, in any room." .


###  http://www.owl-ontologies.com/VirtualHome.owl#tidy
ho:tidy rdf:type owl:Class ;
        rdfs:subClassOf ho:Other ;
        rdfs:comment "The class with sequence of actions for tiding anything." .


###  http://www.owl-ontologies.com/VirtualHome.owl#toast_bread
ho:toast_bread rdf:type owl:Class ;
               rdfs:subClassOf ho:FoodPreparation ;
               rdfs:comment """The class with sequence of actions for toasting the bread (to prepare a 
toast or something else).""" .


###  http://www.owl-ontologies.com/VirtualHome.owl#toilet
ho:toilet rdf:type owl:Class ;
          rdfs:subClassOf ho:HygieneStyling ;
          rdfs:comment "The class with sequence of actions for going to the toilet." .


###  http://www.owl-ontologies.com/VirtualHome.owl#transcribe_what_i_say
ho:transcribe_what_i_say rdf:type owl:Class ;
                         rdfs:subClassOf ho:Work ;
                         rdfs:comment "The class with sequence of actions for trancribe (or copy) the words that I say." .


###  http://www.owl-ontologies.com/VirtualHome.owl#trick_or_treat
ho:trick_or_treat rdf:type owl:Class ;
                  rdfs:subClassOf ho:SocialInteraction ;
                  rdfs:comment "The class with sequence of actions for trick or treat." .


###  http://www.owl-ontologies.com/VirtualHome.owl#try_yourself_off
ho:try_yourself_off rdf:type owl:Class ;
                    rdfs:subClassOf ho:Other ;
                    rdfs:comment """The class with sequence of actions for trying yourself off, with any 
activity in any room.""" .


###  http://www.owl-ontologies.com/VirtualHome.owl#tuck_kids_in_bed
ho:tuck_kids_in_bed rdf:type owl:Class ;
                    rdfs:subClassOf ho:SocialInteraction ;
                    rdfs:comment "A class with sequences to put the kids in bed for sleep, or tell a story." .


###  http://www.owl-ontologies.com/VirtualHome.owl#tummy_time
ho:tummy_time rdf:type owl:Class ;
              rdfs:subClassOf ho:Other ;
              rdfs:comment "The class with sequence of actions for tummy time." .


###  http://www.owl-ontologies.com/VirtualHome.owl#turking
ho:turking rdf:type owl:Class ;
           rdfs:subClassOf ho:Other ;
           rdfs:comment "The class with sequence of actions for turking." .


###  http://www.owl-ontologies.com/VirtualHome.owl#turn_light_off
ho:turn_light_off rdf:type owl:Class ;
                  rdfs:subClassOf ho:Other ;
                  rdfs:comment """The class with sequence of actions for  turning off the light form any 
room.""" .


###  http://www.owl-ontologies.com/VirtualHome.owl#turn_night_light_on
ho:turn_night_light_on rdf:type owl:Class ;
                       rdfs:subClassOf ho:HouseArrangement ;
                       rdfs:comment "The class with sequence of actions for turning the night light on." .


###  http://www.owl-ontologies.com/VirtualHome.owl#turn_off_light
ho:turn_off_light rdf:type owl:Class ;
                  rdfs:subClassOf ho:HouseArrangement ;
                  rdfs:comment "The class with sequence of actions for turning off the lights." .


###  http://www.owl-ontologies.com/VirtualHome.owl#turn_off_tv
ho:turn_off_tv rdf:type owl:Class ;
               rdfs:subClassOf ho:Leisure ;
               rdfs:comment "The class with sequence of actions for turning off the TV." .


###  http://www.owl-ontologies.com/VirtualHome.owl#turn_on_computer
ho:turn_on_computer rdf:type owl:Class ;
                    rdfs:subClassOf ho:Other ;
                    rdfs:comment """The class with sequence of actions for turning on a computer (laptop, or 
personal computer).""" .


###  http://www.owl-ontologies.com/VirtualHome.owl#turn_on_light
ho:turn_on_light rdf:type owl:Class ;
                 rdfs:subClassOf ho:Other ;
                 rdfs:comment """A class with sequences on how to turn on the lights from different 
rooms, and different scenaria such as holding other objects or having to 
stand up from bed.""" .


###  http://www.owl-ontologies.com/VirtualHome.owl#turn_on_lights
ho:turn_on_lights rdf:type owl:Class ;
                  rdfs:subClassOf ho:Other ;
                  rdfs:comment """The class with sequence of actions for turning on the lights more than 
one.""" .


###  http://www.owl-ontologies.com/VirtualHome.owl#turn_on_radio
ho:turn_on_radio rdf:type owl:Class ;
                 rdfs:subClassOf ho:Leisure ;
                 rdfs:comment """The class with sequence of actions for turning on the radio (just 
turning on).
    </p>""" .


###  http://www.owl-ontologies.com/VirtualHome.owl#turn_on_tv
ho:turn_on_tv rdf:type owl:Class ;
              rdfs:subClassOf ho:Leisure ;
              rdfs:comment "The class with sequence of actions on hoe to turn on the TV (just turn on tv, not other actions)." .


###  http://www.owl-ontologies.com/VirtualHome.owl#turn_on_tv_with_remote
ho:turn_on_tv_with_remote rdf:type owl:Class ;
                          rdfs:subClassOf ho:Leisure ;
                          rdfs:comment "The class with sequence of actions for watching tv while using remote control." .


###  http://www.owl-ontologies.com/VirtualHome.owl#type_up_document
ho:type_up_document rdf:type owl:Class ;
                    rdfs:subClassOf ho:Work ;
                    rdfs:comment "The class with sequence of actions for typing up a document." .


###  http://www.owl-ontologies.com/VirtualHome.owl#unload_dishwasher
ho:unload_dishwasher rdf:type owl:Class ;
                     rdfs:subClassOf ho:HouseArrangement ;
                     rdfs:comment "The class with sequence of actions for unloadinf the dishwasher." .


###  http://www.owl-ontologies.com/VirtualHome.owl#unload_various_items_from_pockets_and_place_them_in_bowl_on_table
ho:unload_various_items_from_pockets_and_place_them_in_bowl_on_table rdf:type owl:Class ;
                                                                     rdfs:subClassOf ho:HouseArrangement ;
                                                                     rdfs:comment """The class with sequence of actions for unloading various itmes form 
pockets and place them in bowl on table.""" .


###  http://www.owl-ontologies.com/VirtualHome.owl#update_address_book
ho:update_address_book rdf:type owl:Class ;
                       rdfs:subClassOf ho:Work ;
                       rdfs:comment """The class with sequence of actions that are neede to update your address 
book.""" .


###  http://www.owl-ontologies.com/VirtualHome.owl#use_bathroom
ho:use_bathroom rdf:type owl:Class ;
                rdfs:subClassOf ho:HygieneStyling ;
                rdfs:comment """The class with sequence of actions for using the bathroom, the whole 
room.""" .


###  http://www.owl-ontologies.com/VirtualHome.owl#use_computer
ho:use_computer rdf:type owl:Class ;
                rdfs:subClassOf ho:Work ;
                rdfs:comment "Class wih sequences on how to perform general task with a computer." .


###  http://www.owl-ontologies.com/VirtualHome.owl#use_laptop
ho:use_laptop rdf:type owl:Class ;
              rdfs:subClassOf ho:Other ;
              rdfs:comment """The class with sequence of actions for using your laptop, variety of 
functions.""" .


###  http://www.owl-ontologies.com/VirtualHome.owl#use_restroom
ho:use_restroom rdf:type owl:Class ;
                rdfs:subClassOf ho:HygieneStyling ;
                rdfs:comment "The class with sequence of actions for using the restroom." .


###  http://www.owl-ontologies.com/VirtualHome.owl#use_toilet
ho:use_toilet rdf:type owl:Class ;
              rdfs:subClassOf ho:HygieneStyling ;
              rdfs:comment "The class with sequence of actions for using the toilet." .


###  http://www.owl-ontologies.com/VirtualHome.owl#vacuum_carpet
ho:vacuum_carpet rdf:type owl:Class ;
                 rdfs:subClassOf ho:HouseCleaning ;
                 rdfs:comment "The class with sequence of actions for vacuum the carpet." .


###  http://www.owl-ontologies.com/VirtualHome.owl#visit
ho:visit rdf:type owl:Class ;
         rdfs:subClassOf ho:SocialInteraction ;
         rdfs:comment "The class with sequence of actions for visitng someone elses house." .


###  http://www.owl-ontologies.com/VirtualHome.owl#visit_neighbors
ho:visit_neighbors rdf:type owl:Class ;
                   rdfs:subClassOf ho:SocialInteraction ;
                   rdfs:comment "The class with sequence of actions for visitng neighbors." .


###  http://www.owl-ontologies.com/VirtualHome.owl#visit_with_friends_while_engaging_in_games
ho:visit_with_friends_while_engaging_in_games rdf:type owl:Class ;
                                              rdfs:subClassOf ho:Other ;
                                              rdfs:comment "The class with sequence of actions for visiting friends while engaging in games." .


###  http://www.owl-ontologies.com/VirtualHome.owl#wake_kids_up
ho:wake_kids_up rdf:type owl:Class ;
                rdfs:subClassOf ho:SocialInteraction ;
                rdfs:comment "The class with sequence of actions for waking kids up from sleep." .


###  http://www.owl-ontologies.com/VirtualHome.owl#wake_me_up
ho:wake_me_up rdf:type owl:Class ;
              rdfs:subClassOf ho:BedTimeSleep ;
              rdfs:comment "The class with sequence of actions for telling the system to wake up the user." .


###  http://www.owl-ontologies.com/VirtualHome.owl#walk_through
ho:walk_through rdf:type owl:Class ;
                rdfs:subClassOf ho:Other ;
                rdfs:comment "The class with sequence of actions for walking through a door." .


###  http://www.owl-ontologies.com/VirtualHome.owl#walk_to_room
ho:walk_to_room rdf:type owl:Class ;
                rdfs:subClassOf ho:Other ;
                rdfs:comment "The class with sequence of actions for walking to room, any room." .


###  http://www.owl-ontologies.com/VirtualHome.owl#wash_and_clean_all_crystal_in_china_cabinet
ho:wash_and_clean_all_crystal_in_china_cabinet rdf:type owl:Class ;
                                               rdfs:subClassOf ho:HouseArrangement ;
                                               rdfs:comment """The class with sequence of actions for washing and cleaning all crystal 
in china cabinet.""" .


###  http://www.owl-ontologies.com/VirtualHome.owl#wash_back
ho:wash_back rdf:type owl:Class ;
             rdfs:subClassOf ho:Other ;
             rdfs:comment """The class with sequence of actions for washing back, your own or others 
back.""" .


###  http://www.owl-ontologies.com/VirtualHome.owl#wash_clothes
ho:wash_clothes rdf:type owl:Class ;
                rdfs:subClassOf ho:HouseArrangement ;
                rdfs:comment "Class with sequences for washing clothes." .


###  http://www.owl-ontologies.com/VirtualHome.owl#wash_dining_table
ho:wash_dining_table rdf:type owl:Class ;
                     rdfs:subClassOf ho:Other ;
                     rdfs:comment "The class with sequence of actions for washing dining table." .


###  http://www.owl-ontologies.com/VirtualHome.owl#wash_dirty_dishes
ho:wash_dirty_dishes rdf:type owl:Class ;
                     rdfs:subClassOf ho:HouseCleaning ;
                     rdfs:comment "The class with sequence of actions for washing dirty dishes." .


###  http://www.owl-ontologies.com/VirtualHome.owl#wash_dishes
ho:wash_dishes rdf:type owl:Class ;
               rdfs:subClassOf ho:HouseArrangement ;
               rdfs:comment "The class with sequence of actions for washing up dishes, in the general case or getting ready to wash dishes." .


###  http://www.owl-ontologies.com/VirtualHome.owl#wash_dishes_by_hand
ho:wash_dishes_by_hand rdf:type owl:Class ;
                       rdfs:subClassOf ho:HouseArrangement ;
                       rdfs:comment "The class with sequence of actions for washing yp dishes by hand only." .


###  http://www.owl-ontologies.com/VirtualHome.owl#wash_dishes_with_dishwasher
ho:wash_dishes_with_dishwasher rdf:type owl:Class ;
                               rdfs:subClassOf ho:HouseArrangement ;
                               rdfs:comment "The class with sequence of actions for washing up dishes with dishwasher." .


###  http://www.owl-ontologies.com/VirtualHome.owl#wash_face
ho:wash_face rdf:type owl:Class ;
             rdfs:subClassOf ho:HygieneStyling ;
             rdfs:comment "The class with sequence of actions for washing your face." .


###  http://www.owl-ontologies.com/VirtualHome.owl#wash_hair
ho:wash_hair rdf:type owl:Class ;
             rdfs:subClassOf ho:HygieneStyling ;
             rdfs:comment "The class with sequence of actions for washing your hair." .


###  http://www.owl-ontologies.com/VirtualHome.owl#wash_hands
ho:wash_hands rdf:type owl:Class ;
              rdfs:subClassOf ho:HygieneStyling ;
              rdfs:comment "The class with sequence of actions for washing your hands." .


###  http://www.owl-ontologies.com/VirtualHome.owl#wash_monitor
ho:wash_monitor rdf:type owl:Class ;
                rdfs:subClassOf ho:HouseCleaning ;
                rdfs:comment "The class with sequence of actions for washing a some kind of monitor." .


###  http://www.owl-ontologies.com/VirtualHome.owl#wash_sink
ho:wash_sink rdf:type owl:Class ;
             rdfs:subClassOf ho:HouseCleaning ;
             rdfs:comment "The class with sequence of actions for house cleaning." .


###  http://www.owl-ontologies.com/VirtualHome.owl#wash_table
ho:wash_table rdf:type owl:Class ;
              rdfs:subClassOf ho:HouseCleaning ;
              rdfs:comment "The class with sequence of actions for washing the table." .


###  http://www.owl-ontologies.com/VirtualHome.owl#wash_teeth
ho:wash_teeth rdf:type owl:Class ;
              rdfs:subClassOf ho:HygieneStyling ;
              rdfs:comment "The class with sequence of actions for washing teeth (with water for example)." .


###  http://www.owl-ontologies.com/VirtualHome.owl#watch__horror__movie
ho:watch__horror__movie rdf:type owl:Class ;
                        rdfs:subClassOf ho:Leisure ;
                        rdfs:comment """The class with sequence of actions for watching a horror movie 
specifically.""" .


###  http://www.owl-ontologies.com/VirtualHome.owl#watch_fly
ho:watch_fly rdf:type owl:Class ;
             rdfs:subClassOf ho:Other ;
             rdfs:comment """The class with sequence of actions for watching a fly that has entered a 
room.""" .


###  http://www.owl-ontologies.com/VirtualHome.owl#watch_movie
ho:watch_movie rdf:type owl:Class ;
               rdfs:subClassOf ho:Leisure ;
               rdfs:comment "A class about how to watch a movie either on the TV or laptop." .


###  http://www.owl-ontologies.com/VirtualHome.owl#watch_tv
ho:watch_tv rdf:type owl:Class ;
            rdfs:subClassOf ho:Leisure ;
            rdfs:comment "It contains some subclasses on how to watch TV" .


###  http://www.owl-ontologies.com/VirtualHome.owl#watch_youtube
ho:watch_youtube rdf:type owl:Class ;
                 rdfs:subClassOf ho:Leisure ;
                 rdfs:comment "The class with sequence of actions for wathcing YouTube videos." .


###  http://www.owl-ontologies.com/VirtualHome.owl#water_plants
ho:water_plants rdf:type owl:Class ;
                rdfs:subClassOf ho:HouseArrangement ;
                rdfs:comment "The class with sequence of actions for watering the plants." .


###  http://www.owl-ontologies.com/VirtualHome.owl#wave_at_people_walking_by_through_window
ho:wave_at_people_walking_by_through_window rdf:type owl:Class ;
                                            rdfs:subClassOf ho:SocialInteraction ;
                                            rdfs:comment """The class with sequence of actions for waving at people walking by 
through window.""" .


###  http://www.owl-ontologies.com/VirtualHome.owl#whine
ho:whine rdf:type owl:Class ;
         rdfs:subClassOf ho:Other ;
         rdfs:comment "The class with sequence of actions for whining in any room." .


###  http://www.owl-ontologies.com/VirtualHome.owl#wipe_down_baseboards_please
ho:wipe_down_baseboards_please rdf:type owl:Class ;
                               rdfs:subClassOf ho:Other ;
                               rdfs:comment "The class with sequence of actions for wipe down baseboards please." .


###  http://www.owl-ontologies.com/VirtualHome.owl#wipe_down_counter
ho:wipe_down_counter rdf:type owl:Class ;
                     rdfs:subClassOf ho:Other ;
                     rdfs:comment "The class with sequence of actions for wiping down counter, for any domestic machine that has such." .


###  http://www.owl-ontologies.com/VirtualHome.owl#wipe_down_sink
ho:wipe_down_sink rdf:type owl:Class ;
                  rdfs:subClassOf ho:HouseCleaning ;
                  rdfs:comment """The class with sequence of actions in order to wipe down sink, only this 
part of cleaning not all the cleaning procedure.""" .


###  http://www.owl-ontologies.com/VirtualHome.owl#wipe_feet
ho:wipe_feet rdf:type owl:Class ;
             rdfs:subClassOf ho:HygieneStyling ;
             rdfs:comment "The class with sequence of actions for wiping your own feet." .


###  http://www.owl-ontologies.com/VirtualHome.owl#wipe_off_shoes
ho:wipe_off_shoes rdf:type owl:Class ;
                  rdfs:subClassOf ho:Other ;
                  rdfs:comment "The class with sequence of actions for wiping your shoes off." .


###  http://www.owl-ontologies.com/VirtualHome.owl#wipe_room_down_with_lysol
ho:wipe_room_down_with_lysol rdf:type owl:Class ;
                             rdfs:subClassOf ho:HouseCleaning ;
                             rdfs:comment "The class with sequence of actions for wiping down the room with lysol." .


###  http://www.owl-ontologies.com/VirtualHome.owl#workout
ho:workout rdf:type owl:Class ;
           rdfs:subClassOf ho:PhysicalActivity ;
           rdfs:comment """A class with soft physical activity, or exercise, such as weight 
lifting, workout.""" .


###  http://www.owl-ontologies.com/VirtualHome.owl#write_an_email
ho:write_an_email rdf:type owl:Class ;
                  rdfs:subClassOf ho:Work ;
                  rdfs:comment "The class with sequence of actions for wrtiting ana email." .


###  http://www.owl-ontologies.com/VirtualHome.owl#write_book
ho:write_book rdf:type owl:Class ;
              rdfs:subClassOf ho:Other ;
              rdfs:comment "The class with sequence of actions for writing a book, in any room." .


###  http://www.owl-ontologies.com/VirtualHome.owl#write_in_your_diary
ho:write_in_your_diary rdf:type owl:Class ;
                       rdfs:subClassOf ho:Other ;
                       rdfs:comment """The class with sequence of actions for writing in your diary, in any 
room.""" .


###  http://www.owl-ontologies.com/VirtualHome.owl#write_letter
ho:write_letter rdf:type owl:Class ;
                rdfs:subClassOf ho:Work ;
                rdfs:comment "Class with sequences on how to write a letter." .


###  http://www.owl-ontologies.com/VirtualHome.owl#write_report
ho:write_report rdf:type owl:Class ;
                rdfs:subClassOf ho:Work ;
                rdfs:comment "The class with sequence of actions for writing some kind of report." .


###  http://www.owl-ontologies.com/VirtualHome.owl#write_research_paper
ho:write_research_paper rdf:type owl:Class ;
                        rdfs:subClassOf ho:Work ;
                        rdfs:comment "The class with sequence of actions for writing a research paper." .


###  http://www.owl-ontologies.com/VirtualHome.owl#write_research_papers
ho:write_research_papers rdf:type owl:Class ;
                         rdfs:subClassOf ho:Work ;
                         rdfs:comment """The class with sequence of actions for writing reaseach papers (only 
research paper).""" .


###  http://www.owl-ontologies.com/VirtualHome.owl#write_school_paper
ho:write_school_paper rdf:type owl:Class ;
                      rdfs:subClassOf ho:Work ;
                      rdfs:comment """The class with sequence of actions writing school papers, it should not 
be confused with research paper.""" .


###  http://www.owl-ontologies.com/VirtualHome.owl#write_story
ho:write_story rdf:type owl:Class ;
               rdfs:subClassOf ho:Other ;
               rdfs:comment """The class with sequence of actions for writing a story, on the computer 
or on paper.""" .


###  http://www.owl-ontologies.com/VirtualHome.owl#write_thank_you_notes
ho:write_thank_you_notes rdf:type owl:Class ;
                         rdfs:subClassOf ho:Work ;
                         rdfs:comment "The class with sequence of actions to write a thank you note to somebody." .


###  http://www.owl-ontologies.com/VirtualHome.owl#yoga
ho:yoga rdf:type owl:Class ;
        rdfs:subClassOf ho:PhysicalActivity ;
        rdfs:comment "The class with sequence of actions for doing yoga." .


###  http://www.w3.org/2006/time#Duration
<http://www.w3.org/2006/time#Duration> rdf:type owl:Class .


###  http://www.w3.org/2006/time#TemporalUnit
<http://www.w3.org/2006/time#TemporalUnit> rdf:type owl:Class .


###  https://www.web3d.org/specifications/X3dOntology4.0#SFDouble
x3do:SFDouble rdf:type owl:Class ;
              rdfs:subClassOf x3do:X3DField .


###  https://www.web3d.org/specifications/X3dOntology4.0#SFVec3f
x3do:SFVec3f rdf:type owl:Class ;
             rdfs:subClassOf x3do:X3DField .


###  https://www.web3d.org/specifications/X3dOntology4.0#Shape
x3do:Shape rdf:type owl:Class ;
           rdfs:comment "used for 3D bounding box" .

[ rdf:type owl:Axiom ;
   owl:annotatedSource x3do:Shape ;
   owl:annotatedProperty rdfs:comment ;
   owl:annotatedTarget "used for 3D bounding box" ;
   rdfs:comment "commented by vh2kg_ontology"
 ] .


###  https://www.web3d.org/specifications/X3dOntology4.0#X3DField
x3do:X3DField rdf:type owl:Class ;
              rdfs:comment "X3DField is the abstract field type from which all single-valued field types are derived." .


#################################################################
#    Individuals
#################################################################

###  http://example.org/virtualhome2kg/ontology/BODY_PART
:BODY_PART rdf:type owl:NamedIndividual .


###  http://example.org/virtualhome2kg/ontology/CAN_OPEN
:CAN_OPEN rdf:type owl:NamedIndividual ,
                   :Affordance ;
          :affordAction :Open .


###  http://example.org/virtualhome2kg/ontology/CLEAN
:CLEAN rdf:type owl:NamedIndividual ,
                :StateType .


###  http://example.org/virtualhome2kg/ontology/CLOSED
:CLOSED rdf:type owl:NamedIndividual ,
                 :StateType .


###  http://example.org/virtualhome2kg/ontology/CLOTHES
:CLOTHES rdf:type owl:NamedIndividual .


###  http://example.org/virtualhome2kg/ontology/CONTAINERS
:CONTAINERS rdf:type owl:NamedIndividual .


###  http://example.org/virtualhome2kg/ontology/COVER_OBJECT
:COVER_OBJECT rdf:type owl:NamedIndividual .


###  http://example.org/virtualhome2kg/ontology/CREAM
:CREAM rdf:type owl:NamedIndividual ,
                :Attribute .


###  http://example.org/virtualhome2kg/ontology/CUTTABLE
:CUTTABLE rdf:type owl:NamedIndividual ,
                   :Affordance ;
          :affordAction :Cut .


###  http://example.org/virtualhome2kg/ontology/Cut
:Cut rdf:type owl:NamedIndividual .


###  http://example.org/virtualhome2kg/ontology/DIRTY
:DIRTY rdf:type owl:NamedIndividual ,
                :StateType .


###  http://example.org/virtualhome2kg/ontology/DRINKABLE
:DRINKABLE rdf:type owl:NamedIndividual ,
                    :Affordance ;
           :affordAction :Drink .


###  http://example.org/virtualhome2kg/ontology/Drink
:Drink rdf:type owl:NamedIndividual .


###  http://example.org/virtualhome2kg/ontology/EATABLE
:EATABLE rdf:type owl:NamedIndividual ,
                  :Affordance ;
         :affordAction :Eat .


###  http://example.org/virtualhome2kg/ontology/Eat
:Eat rdf:type owl:NamedIndividual .


###  http://example.org/virtualhome2kg/ontology/GRABBABLE
:GRABBABLE rdf:type owl:NamedIndividual ,
                    :Affordance ;
           :affordAction :Grab .


###  http://example.org/virtualhome2kg/ontology/Grab
:Grab rdf:type owl:NamedIndividual .


###  http://example.org/virtualhome2kg/ontology/HANGABLE
:HANGABLE rdf:type owl:NamedIndividual ,
                   :Affordance ;
          :affordAction :PutBack ,
                        :PutOff .


###  http://example.org/virtualhome2kg/ontology/HAS_PAPER
:HAS_PAPER rdf:type owl:NamedIndividual ,
                    :Attribute .


###  http://example.org/virtualhome2kg/ontology/HAS_PLUG
:HAS_PLUG rdf:type owl:NamedIndividual ,
                   :Attribute .


###  http://example.org/virtualhome2kg/ontology/HAS_SWITCH
:HAS_SWITCH rdf:type owl:NamedIndividual ,
                     :Attribute .


###  http://example.org/virtualhome2kg/ontology/LIEABLE
:LIEABLE rdf:type owl:NamedIndividual ,
                  :Affordance ;
         :affordAction :Lie .


###  http://example.org/virtualhome2kg/ontology/LOOKABLE
:LOOKABLE rdf:type owl:NamedIndividual ,
                   :Affordance ;
          :affordAction :Watch .


###  http://example.org/virtualhome2kg/ontology/LYING
:LYING rdf:type owl:NamedIndividual ,
                :StateType .


###  http://example.org/virtualhome2kg/ontology/Lie
:Lie rdf:type owl:NamedIndividual .


###  http://example.org/virtualhome2kg/ontology/MOVABLE
:MOVABLE rdf:type owl:NamedIndividual ,
                  :Affordance ;
         :affordAction :Move .


###  http://example.org/virtualhome2kg/ontology/Move
:Move rdf:type owl:NamedIndividual .


###  http://example.org/virtualhome2kg/ontology/OFF
:OFF rdf:type owl:NamedIndividual ,
              :StateType .


###  http://example.org/virtualhome2kg/ontology/ON
:ON rdf:type owl:NamedIndividual ,
             :StateType .


###  http://example.org/virtualhome2kg/ontology/OPEN
:OPEN rdf:type owl:NamedIndividual ,
               :StateType .


###  http://example.org/virtualhome2kg/ontology/Open
:Open rdf:type owl:NamedIndividual .


###  http://example.org/virtualhome2kg/ontology/PERSON
:PERSON rdf:type owl:NamedIndividual ,
                 :Attribute .


###  http://example.org/virtualhome2kg/ontology/PLUGGED_IN
:PLUGGED_IN rdf:type owl:NamedIndividual ,
                     :StateType .


###  http://example.org/virtualhome2kg/ontology/PLUGGED_OUT
:PLUGGED_OUT rdf:type owl:NamedIndividual ,
                      :StateType .


###  http://example.org/virtualhome2kg/ontology/POURABLE
:POURABLE rdf:type owl:NamedIndividual ,
                   :Affordance ;
          :affordAction :Pour .


###  http://example.org/virtualhome2kg/ontology/Pour
:Pour rdf:type owl:NamedIndividual .


###  http://example.org/virtualhome2kg/ontology/PutBack
:PutBack rdf:type owl:NamedIndividual .


###  http://example.org/virtualhome2kg/ontology/PutOff
:PutOff rdf:type owl:NamedIndividual .


###  http://example.org/virtualhome2kg/ontology/READABLE
:READABLE rdf:type owl:NamedIndividual ,
                   :Affordance ;
          :affordAction :Read .


###  http://example.org/virtualhome2kg/ontology/RECIPIENT
:RECIPIENT rdf:type owl:NamedIndividual ,
                    :Attribute .


###  http://example.org/virtualhome2kg/ontology/Read
:Read rdf:type owl:NamedIndividual .


###  http://example.org/virtualhome2kg/ontology/SITTABLE
:SITTABLE rdf:type owl:NamedIndividual ,
                   :Affordance ;
          :affordAction :Sit .


###  http://example.org/virtualhome2kg/ontology/SITTING
:SITTING rdf:type owl:NamedIndividual ,
                  :StateType .


###  http://example.org/virtualhome2kg/ontology/SURFACES
:SURFACES rdf:type owl:NamedIndividual ,
                   :Attribute .


###  http://example.org/virtualhome2kg/ontology/Sit
:Sit rdf:type owl:NamedIndividual .


###  http://example.org/virtualhome2kg/ontology/Watch
:Watch rdf:type owl:NamedIndividual .


###  http://www.w3.org/2006/time#unitSecond
<http://www.w3.org/2006/time#unitSecond> rdf:type owl:NamedIndividual ,
                                                  <http://www.w3.org/2006/time#TemporalUnit> .


#################################################################
#    Annotations
#################################################################

x3do:SFDouble <http://purl.org/dc/terms/description> "SFDouble is a double-precision floating-point type. Array values are optionally separated by commas in XML syntax. See GeoVRML 1.0 Recommended Practice, Section 2.3, Limitations of Single Precision for rationale." .


x3do:SFVec3f <http://purl.org/dc/terms/description> "SFVec3d is a 3-tuple triplet of SFDouble values. See GeoVRML 1.0 Recommended Practice, Section 2.3, Limitations of Single Precision. Hint: SFVec3d can be used to specify a georeferenced 3D coordinate. Warning: comma characters within singleton values do not pass strict XML validation." .


###  Generated by the OWL API (version 4.5.9.2019-02-01T07:24:44Z) https://github.com/owlcs/owlapi
